WIP in inline proof

theories/L6_PCPS/inline_correct_alt.v
@@ -389,7 +389,7 @@ Section Inline_correct.
     fun x => exists f ft xs e, fm ! f = Some (ft, xs, e) /\ x \in occurs_free e \\ FromList xs.
 
   Definition bound_var_fun_map (fm : fun_map) : Ensemble var :=
-    fun x => exists f ft xs e, fm ! f = Some (ft, xs, e) /\ x \in bound_var e \\ funnames_in_exp e :|: FromList xs.
+    fun x => exists f ft xs e, fm ! f = Some (ft, xs, e) /\ x \in bound_var e :|: FromList xs.
 
 
   Lemma occurs_free_fun_map_get f ft xs e (fm : fun_map) :
@@ -414,24 +414,25 @@ Section Inline_correct.
 
   Lemma bound_var_fun_map_get f ft xs e (fm : fun_map) :
     M.get f fm = Some (ft, xs, e) ->
-    bound_var e \\ funnames_in_exp e :|: (FromList xs) \subset bound_var_fun_map fm.
+    bound_var e :|: (FromList xs) \subset bound_var_fun_map fm.
   Proof.
     intros Hget z Hin. do 4 eexists. split; eauto.
   Qed.
 
   Lemma bound_var_fun_map_add_fundefs_un B fm :
     unique_bindings_fundefs B ->
-    bound_var_fun_map (add_fundefs B fm) \subset (bound_var_fundefs B \\ funnames_in_fundefs B \\ name_in_fundefs B) :|: bound_var_fun_map fm.
+    bound_var_fun_map (add_fundefs B fm) \subset (bound_var_fundefs B \\ name_in_fundefs B) :|: bound_var_fun_map fm.
   Proof.
     intros Hun x [z Hin]. destructAll. destruct (Decidable_name_in_fundefs B). destruct (Dec z).
     - edestruct name_in_fundefs_find_def_is_Some. eassumption. destructAll. erewrite add_fundefs_in in H; [| eassumption ]. inv H.
       edestruct unique_bindings_fun_in_fundefs. eapply find_def_correct. eassumption. eassumption. destructAll.
       left.     
       inv H0.
-      + eapply fun_in_fundefs_bound_var_Setminus'.
-        eapply find_def_correct. eassumption. eassumption. eassumption.
-      + eapply fun_in_fundefs_FromList_subset.
-        eapply find_def_correct. eassumption. eassumption. eassumption.
+      + constructor. eapply fun_in_fundefs_bound_var_fundefs. eapply find_def_correct. eassumption. now sets.
+        intros hc. eapply H4; constructor; eauto.
+      + constructor.
+        eapply fun_in_fundefs_bound_var_fundefs. eapply find_def_correct. eassumption. now sets.
+        intros hc. eapply H5; constructor; eauto.
     - right. rewrite add_fundefs_not_in in H. do 4 eexists; split; eauto.
       eassumption.
   Qed. 
@@ -463,7 +464,7 @@ Section Inline_correct.
   Lemma bound_var_fun_map_remove_add_fundefs_un' (B : fundefs) (fm : fun_map) f :
     unique_bindings_fundefs B ->
     bound_var_fun_map (M.remove f (add_fundefs B fm)) \subset
-    bound_var_fundefs B \\ funnames_in_fundefs B \\ name_in_fundefs B :|: bound_var_fun_map (M.remove f fm).
+    bound_var_fundefs B \\ name_in_fundefs B :|: bound_var_fun_map (M.remove f fm).
   Proof.
     intros Hun x [z Hin]. destructAll. destruct (peq f z); subst.
     - rewrite M.grs in H. inv H.
@@ -473,74 +474,75 @@ Section Inline_correct.
         edestruct unique_bindings_fun_in_fundefs. eapply find_def_correct. eassumption. eassumption. destructAll.
         left.     
         inv H0.
-        * eapply fun_in_fundefs_bound_var_Setminus'.
-          eapply find_def_correct. eassumption. eassumption. eassumption.
-        * eapply fun_in_fundefs_FromList_subset.
-          eapply find_def_correct. eassumption. eassumption. eassumption.
+        * constructor. eapply fun_in_fundefs_bound_var_fundefs. eapply find_def_correct. eassumption. now sets.
+          intros hc. eapply H4; constructor; eauto.
+        * constructor.
+          eapply fun_in_fundefs_bound_var_fundefs. eapply find_def_correct. eassumption. now sets.
+          intros hc. eapply H5; constructor; eauto.          
       + right. rewrite add_fundefs_not_in in H. do 4 eexists; split; eauto.
         rewrite M.gro; now eauto. eassumption.
   Qed. 
 
-  (* Lemma bound_var_fun_map_remove_add_fundefs_un (B : fundefs) (fm : fun_map) f ft xs e: *)
-  (*   unique_bindings_fundefs B -> *)
-  (*   find_def f B = Some (ft, xs, e) -> *)
-  (*   bound_var_fun_map (M.remove f (add_fundefs B fm)) \subset *)
-  (*   bound_var_fundefs B \\ funnames_in_fundefs B \\ name_in_fundefs B \\ bound_var e \\ FromList xs :|: bound_var_fun_map (M.remove f fm). *)
-  (* Proof. *)
-  (*   induction B. *)
-  (*   - intros Hun Hfind. inv Hun. destruct (peq f v); subst. *)
-  (*     + simpl in *. rewrite peq_true in Hfind. inv Hfind.  *)
-  (*       intros x [z Hin]. destructAll. rewrite remove_set_1 in H. *)
-  (*       destruct (peq v z); subst. *)
-  (*       * rewrite M.grs in H. inv H. *)
-  (*       * rewrite M.gro in H; eauto. destruct (Decidable_name_in_fundefs B). destruct (Dec z). *)
-  (*         -- edestruct name_in_fundefs_find_def_is_Some. eassumption. destructAll.  *)
-  (*            erewrite add_fundefs_in in H; [| eassumption ]. inv H. normalize_bound_var. simpl. *)
-  (*            edestruct unique_bindings_fun_in_fundefs. eapply find_def_correct. eassumption. eassumption. destructAll. *)
+  Lemma bound_var_fun_map_remove_add_fundefs_un (B : fundefs) (fm : fun_map) f ft xs e:
+    unique_bindings_fundefs B ->
+    find_def f B = Some (ft, xs, e) ->
+    bound_var_fun_map (M.remove f (add_fundefs B fm)) \subset
+    bound_var_fundefs B \\ name_in_fundefs B \\ bound_var e \\ FromList xs :|: bound_var_fun_map (M.remove f fm).
+  Proof.
+    induction B.
+    - intros Hun Hfind. inv Hun. destruct (peq f v); subst.
+      + simpl in *. rewrite peq_true in Hfind. inv Hfind. 
+        intros x [z Hin]. destructAll. rewrite remove_set_1 in H.
+        destruct (peq v z); subst.
+        * rewrite M.grs in H. inv H.
+        * rewrite M.gro in H; eauto. destruct (Decidable_name_in_fundefs B). destruct (Dec z).
+          -- edestruct name_in_fundefs_find_def_is_Some. eassumption. destructAll. 
+             erewrite add_fundefs_in in H; [| eassumption ]. inv H. normalize_bound_var. simpl.
+             edestruct unique_bindings_fun_in_fundefs. eapply find_def_correct. eassumption. eassumption. destructAll.
              
-  (*            left. constructor. constructor. constructor. do 3 right. *)
-  (*             eapply fun_in_fundefs_bound_var_fundefs. eapply find_def_correct. eassumption. inv H0; now eauto. *)
-  (*            ++ intros Hc; inv Hc; eauto. inv H17. eapply H5.  *)
-  (*               eapply fun_in_fundefs_bound_var_fundefs. eapply find_def_correct. eassumption. inv H0; now eauto. *)
-  (*               inv H0; eauto. eapply H13; constructor. eassumption. eassumption. *)
-  (*               eapply H14; constructor. eassumption. eassumption. *)
-  (*            ++ intros hc. eapply H8. constructor. eassumption. eapply fun_in_fundefs_bound_var_fundefs. eapply find_def_correct. eassumption. *)
-  (*               inv H0; eauto. *)
-  (*            ++ intros hc. eapply H7. constructor. eapply fun_in_fundefs_bound_var_fundefs. eapply find_def_correct. eassumption. *)
-  (*               inv H0; eauto. eassumption. *)
-  (*         -- rewrite add_fundefs_not_in in H; eauto. right. do 4 eexists. split. rewrite M.gro. eassumption. now eauto. *)
-  (*            eassumption. *)
-  (*     + simpl in Hfind. rewrite peq_false in Hfind; eauto. assert (Hf' := Hfind). eapply IHB in Hfind; eauto. *)
-  (*       simpl. intros x Hin. destruct Hin. destructAll. normalize_bound_var. simpl. *)
-  (*       destruct (peq f x0); subst. *)
-  (*       * rewrite M.grs in H. inv H. *)
-  (*       * rewrite M.gro in H; eauto. destruct (peq v x0). subst. *)
-  (*         -- rewrite M.gss in H. inv H. left. constructor. constructor. constructor. *)
-  (*            inv H0; now eauto. *)
-  (*            ++ intros Hc. inv Hc. inv H. now inv H0; eauto. *)
-  (*               inv H0. eapply H8. constructor. eassumption. eapply name_in_fundefs_bound_var_fundefs. eassumption. *)
-  (*               eapply H7. constructor. eapply name_in_fundefs_bound_var_fundefs. eassumption. eassumption. *)
-  (*            ++ intros Hc1. inv H0. eapply H8. constructor. eassumption.  *)
-  (*               eapply fun_in_fundefs_bound_var_fundefs. eapply find_def_correct. eassumption. now eauto. *)
-  (*               eapply H7. constructor. *)
-  (*               eapply fun_in_fundefs_bound_var_fundefs. eapply find_def_correct. eassumption. now eauto. *)
-  (*               eassumption. *)
-  (*            ++ intros Hc1. inv H0. eapply H8. constructor. eassumption.  *)
-  (*               eapply fun_in_fundefs_bound_var_fundefs. eapply find_def_correct. eassumption. now eauto. *)
-  (*               eapply H7. constructor. *)
-  (*               eapply fun_in_fundefs_bound_var_fundefs. eapply find_def_correct. eassumption. now eauto. *)
-  (*               eassumption. *)
-  (*         -- rewrite M.gso in H.          *)
-  (*            assert (Hin' : x \in bound_var_fun_map (M.remove f (add_fundefs B fm))). *)
-  (*            { do 4 eexists. split. rewrite M.gro. eassumption. now eauto. eassumption. } *)
-  (*            eapply Hfind in Hin'. inv Hin'; [| now eauto ]. left. inv H1. inv H2. inv H1.  *)
-  (*            constructor. constructor. constructor. eauto. *)
-  (*            ++ intros Hc; inv Hc; eauto. inv H1. contradiction. *)
-  (*            ++ eassumption. *)
-  (*            ++ eassumption. *)
-  (*            ++ eauto. *)
-  (*   - intros. inv H0. *)
-  (* Qed.  *)
+             left. constructor. constructor. constructor. do 3 right.
+              eapply fun_in_fundefs_bound_var_fundefs. eapply find_def_correct. eassumption. inv H0; now eauto.
+             ++ intros Hc; inv Hc; eauto. inv H17. eapply H5. 
+                eapply fun_in_fundefs_bound_var_fundefs. eapply find_def_correct. eassumption. inv H0; now eauto.
+                inv H0; eauto. eapply H13; constructor. eassumption. eassumption.
+                eapply H14; constructor. eassumption. eassumption.
+             ++ intros hc. eapply H8. constructor. eassumption. eapply fun_in_fundefs_bound_var_fundefs. eapply find_def_correct. eassumption.
+                inv H0; eauto.
+             ++ intros hc. eapply H7. constructor. eapply fun_in_fundefs_bound_var_fundefs. eapply find_def_correct. eassumption.
+                inv H0; eauto. eassumption.
+          -- rewrite add_fundefs_not_in in H; eauto. right. do 4 eexists. split. rewrite M.gro. eassumption. now eauto.
+             eassumption.
+      + simpl in Hfind. rewrite peq_false in Hfind; eauto. assert (Hf' := Hfind). eapply IHB in Hfind; eauto.
+        simpl. intros x Hin. destruct Hin. destructAll. normalize_bound_var. simpl.
+        destruct (peq f x0); subst.
+        * rewrite M.grs in H. inv H.
+        * rewrite M.gro in H; eauto. destruct (peq v x0). subst.
+          -- rewrite M.gss in H. inv H. left. constructor. constructor. constructor.
+             inv H0; now eauto.
+             ++ intros Hc. inv Hc. inv H. now inv H0; eauto.
+                inv H0. eapply H8. constructor. eassumption. eapply name_in_fundefs_bound_var_fundefs. eassumption.
+                eapply H7. constructor. eapply name_in_fundefs_bound_var_fundefs. eassumption. eassumption.
+             ++ intros Hc1. inv H0. eapply H8. constructor. eassumption. 
+                eapply fun_in_fundefs_bound_var_fundefs. eapply find_def_correct. eassumption. now eauto.
+                eapply H7. constructor.
+                eapply fun_in_fundefs_bound_var_fundefs. eapply find_def_correct. eassumption. now eauto.
+                eassumption.
+             ++ intros Hc1. inv H0. eapply H8. constructor. eassumption. 
+                eapply fun_in_fundefs_bound_var_fundefs. eapply find_def_correct. eassumption. now eauto.
+                eapply H7. constructor.
+                eapply fun_in_fundefs_bound_var_fundefs. eapply find_def_correct. eassumption. now eauto.
+                eassumption.
+          -- rewrite M.gso in H.         
+             assert (Hin' : x \in bound_var_fun_map (M.remove f (add_fundefs B fm))).
+             { do 4 eexists. split. rewrite M.gro. eassumption. now eauto. eassumption. }
+             eapply Hfind in Hin'. inv Hin'; [| now eauto ]. left. inv H1. inv H2. inv H1. 
+             constructor. constructor. constructor. eauto.
+             ++ intros Hc; inv Hc; eauto. inv H1. contradiction.
+             ++ eassumption.
+             ++ eassumption.
+             ++ eauto.
+    - intros. inv H0.
+  Qed. 
 
   Lemma  bound_var_fun_map_remove f fm :
     bound_var_fun_map (M.remove f fm) \subset bound_var_fun_map fm.
@@ -998,28 +1000,24 @@ Section Inline_correct.
     destruct k'; eauto. rewrite <- fun_map_inv_eq in *. eapply IHk; eauto.
   Qed.
 
-
-
-  (* [fun_map_vars] *)  
   Definition fun_map_vars (fm : fun_map) (F : Ensemble var) (sig : subst) :=
     forall f ft xs e,
       fm ! f = Some (ft, xs, e) ->
       unique_bindings e /\
       NoDup xs /\
-      Disjoint _ (bound_var e) (FromList xs :|: occurs_free e) /\ 
-      Disjoint _ (bound_var e \\ funnames_in_exp e) (Dom_map fm) /\
+      Disjoint _ (bound_var e) (FromList xs :|: occurs_free e) /\
+      Disjoint _ (bound_var e) (Dom_map fm) /\
       Disjoint _ (bound_var e :|: FromList xs) (occurs_free_fun_map (M.remove f fm)) /\
-      Disjoint _ (funnames_in_exp e) (bound_var_fun_map (M.remove f fm)) /\
+      Disjoint _ (bound_var e :|: occurs_free e) (bound_var_fun_map (M.remove f fm)) /\      
       Disjoint _ (FromList xs) (Dom_map fm) /\      
-      Disjoint _ F (bound_var e :|: image (apply_r sig) (occurs_free e \\ FromList xs)).
+      Disjoint _ F ((* bound_var e :|: *) image (apply_r sig) (occurs_free e \\ FromList xs)).
 
-  
   Lemma fun_map_vars_antimon fm F F' sig :
     fun_map_vars fm F sig ->
     F' \subset F ->
     fun_map_vars fm F' sig.
   Proof.
-    intros Hfm Hsub; intro; intros. eapply Hfm in H. destructAll. 
+    intros Hfm Hsub; intro; intros. eapply Hfm in H. destructAll.
     do 6 (split; eauto). sets.
   Qed.
 
@@ -1036,10 +1034,10 @@ Section Inline_correct.
     fun_map_vars fm (F \\ [set v]) (M.set x v sig).
   Proof.
     intros Hfm; intro; intros. eapply Hfm in H. destructAll.
-    split; [| split; [| split; [| split; [| split; [| split; [| split ]]]]]]; eauto.
-
-    eapply Disjoint_Included_r. eapply Included_Union_compat. reflexivity.
-    eapply image_apply_r_set. xsets.
+    do 8 (split; eauto).
+    (* eapply Union_Disjoint_r. now sets. *)
+    eapply Disjoint_Included_r. eapply image_apply_r_set.
+    eapply Union_Disjoint_r. now sets. now xsets.
   Qed.
   
   Lemma fun_map_vars_set_list fm F sig xs vs :
@@ -1056,22 +1054,22 @@ Section Inline_correct.
         simpl. eapply IHxs; eauto.
   Qed.
 
-
+ 
   Lemma fun_map_vars_def_funs fm S sig B xs :
     fun_map_vars fm S sig ->
     unique_bindings_fundefs B ->
 
-    Disjoint _ (bound_var_fundefs B) (occurs_free_fundefs B :|: occurs_free_fun_map fm) ->    
-    Disjoint _ (bound_var_fundefs B \\ funnames_in_fundefs B \\ name_in_fundefs B) (Dom_map fm) ->
-    Disjoint _ (S \\ FromList xs) (bound_var_fundefs B :|: image (apply_r sig) (occurs_free_fundefs B)) ->    
-    Disjoint _ (name_in_fundefs B :|: funnames_in_fundefs B) (bound_var_fun_map fm) ->
+    Disjoint _ (bound_var_fundefs B) (occurs_free_fundefs B :|: occurs_free_fun_map fm) ->
+    Disjoint _ (occurs_free_fundefs B :|: bound_var_fundefs B) (bound_var_fun_map fm) ->
+    
+    Disjoint _ (bound_var_fundefs B) (Dom_map fm) ->
+    Disjoint _ (S \\ FromList xs) ((* bound_var_fundefs B :|: *) image (apply_r sig) (occurs_free_fundefs B)) ->    
     
     Datatypes.length (all_fun_name B) = Datatypes.length xs ->
     
     fun_map_vars (add_fundefs B fm) (S \\ FromList xs) (set_list (combine (all_fun_name B) xs) sig).
   Proof.
-    intros Hfm Hun Hdis1 Hdis2 Hdis3 Hdis4 Hlen x ft ys e Hget.
-    destruct (Decidable_name_in_fundefs B). destruct (Dec x).
+    intros Hfm Hun Hdis1 Hdis' Hdis2 Hdis3 (* Hdis4 Hdis5 *) Hlen x ft ys e Hget. destruct (Decidable_name_in_fundefs B). destruct (Dec x).
     - edestruct name_in_fundefs_find_def_is_Some; eauto. destructAll. erewrite add_fundefs_in in Hget; eauto.
       inv Hget. edestruct unique_bindings_fun_in_fundefs. eapply find_def_correct. eassumption. eassumption. destructAll.
       assert (Hin1 : bound_var e \subset bound_var_fundefs B).
@@ -1079,56 +1077,54 @@ Section Inline_correct.
       assert (Hin2 : FromList ys \subset bound_var_fundefs B).
       { eapply Included_trans; [| eapply fun_in_fundefs_bound_var_fundefs; eapply find_def_correct; eauto ]. now sets. }
       
-      split. now eauto. split. now eauto. split; [| split; [| split; [| split; [| split ]]]].
+      split. now eauto. split. now eauto. split; [| split; [| split; [| split; [| split; [| split ]]]]].
       + eapply Union_Disjoint_r. now sets.
         eapply fun_in_fundefs_Disjoint_bound_Var_occurs_free. eapply find_def_correct. eassumption.
         eassumption. clear Hdis2. sets.
       + rewrite Dom_map_add_fundefs. eapply Union_Disjoint_r. now sets.
         eapply Disjoint_Included; [| | eapply Hdis2 ]. now sets.
-        eapply fun_in_fundefs_bound_var_Setminus'.
-        eapply find_def_correct. eassumption. eassumption.
-      + eapply Disjoint_Included_r. eapply occurs_free_fun_map_remove_add_fundefs.
-        eapply Union_Disjoint_r; [ eapply Union_Disjoint_r | ]; sets.
-        * eapply Disjoint_Included; [| | eapply Hdis1 ]. now sets.
-          
-          eapply Included_trans; [| eapply fun_in_fundefs_bound_var_fundefs; eapply find_def_correct; eauto ].
-          now sets.
+        eapply Included_trans; [| eapply fun_in_fundefs_bound_var_fundefs; eapply find_def_correct; eauto ]. now sets.
+      + eapply Disjoint_Included_r. eapply occurs_free_fun_map_remove_add_fundefs. eapply Union_Disjoint_r; [ eapply Union_Disjoint_r | ].
+        * eapply Disjoint_Included_l. eapply Union_Included. eassumption.
+          eapply Included_trans; [| eapply fun_in_fundefs_bound_var_fundefs; eapply find_def_correct; eauto ]. now sets.
+          clear Hdis2. sets.
+        * sets.
         * eapply Disjoint_Included_r. eapply occurs_free_fun_map_remove.
-          eapply Disjoint_Included_l.
-          eapply Included_trans; [| eapply fun_in_fundefs_bound_var_fundefs; eapply find_def_correct; eauto ].
-          now sets. now sets.
-      + eapply Disjoint_Included_r.
-        eapply bound_var_fun_map_remove_add_fundefs_un'. eassumption. eapply Union_Disjoint_r.
-        * eapply Disjoint_Included_l. eapply fun_in_fundefs_funnames_in_exp. eapply find_def_correct. eassumption.
-          sets.
-        * eapply Disjoint_Included_r. eapply bound_var_fun_map_remove.
-          eapply Disjoint_Included_l. eapply fun_in_fundefs_funnames_in_exp. eapply find_def_correct. eassumption.
-          sets.
+          eapply Disjoint_Included_l. eapply Union_Included; eassumption. clear Hdis2. sets.
+      + eapply Disjoint_Included_l.
+        * eapply Included_Union_compat. reflexivity. eapply occurs_free_in_fun. eapply find_def_correct. eassumption.
+        * rewrite Union_assoc. eapply Union_Disjoint_l.
+          -- eapply Disjoint_Included_r.
+             eapply bound_var_fun_map_remove_add_fundefs_un. eassumption. eassumption. eapply Union_Disjoint_r.
+             ++ sets.
+             ++ eapply Disjoint_Included. eapply bound_var_fun_map_remove.
+                eapply Union_Included; eassumption. sets.
+          -- eapply Disjoint_Included_r. eapply bound_var_fun_map_remove_add_fundefs_un'. eassumption.
+             eapply Union_Disjoint_r.
+             ++ eapply Union_Disjoint_l. now sets. clear Hdis2. sets.
+             ++ eapply Disjoint_Included_r. eapply bound_var_fun_map_remove.
+                eapply Union_Disjoint_l; [| now sets ]. eapply Disjoint_Included_l.
+                eapply name_in_fundefs_bound_var_fundefs. sets.
       + rewrite Dom_map_add_fundefs. eapply Union_Disjoint_r. eassumption.
         eapply Disjoint_Included_l.
-        eapply fun_in_fundefs_FromList_subset. eapply find_def_correct. eassumption. eassumption.
-        eassumption.
-      + eapply Union_Disjoint_r. now sets. eapply Disjoint_Included_r.
-        * eapply image_apply_r_set_list. now eauto.
-        * SearchAbout ys. eapply Union_Disjoint_r. now sets.
-          rewrite <- Same_set_all_fun_name.
-          eapply Disjoint_Included; [| | eapply Hdis3 ]; [| now sets ].
-          eapply Included_Union_preserv_r. eapply image_monotonic. do 2 eapply Setminus_Included_Included_Union.
-          eapply Included_trans. eapply occurs_free_in_fun. eapply find_def_correct. eassumption. now sets.
+        eapply Included_Setminus. eassumption. eassumption. sets.
+      + (* eapply Union_Disjoint_r. now sets. *)
+        eapply Disjoint_Included_r.
+        eapply image_apply_r_set_list. now eauto. eapply Union_Disjoint_r. now sets.
+        rewrite <- Same_set_all_fun_name.
+        eapply Disjoint_Included; [| | eapply Hdis3 ]; [| now sets ].
+        eapply image_monotonic. do 2 eapply Setminus_Included_Included_Union.
+        eapply Included_trans. eapply occurs_free_in_fun. eapply find_def_correct. eassumption. now sets.
     - rewrite add_fundefs_not_in in Hget; eauto. edestruct Hfm. eassumption. destructAll.
-      split; eauto. split; eauto. split; [| split; [| split; [| split; [| split(* ; [| split ] *)]]]].
+      split; eauto. split; eauto. split; [| split; [| split; [| split; [| split; [| split ]]]]].
       + now sets.
       + rewrite Dom_map_add_fundefs. eapply Union_Disjoint_r.
-        * eapply Disjoint_sym. eapply Disjoint_Included; [| | eapply Hdis4 ].
-          eapply Included_trans; [| eapply bound_var_fun_map_get; eauto ]. now sets. now sets.
+        * eapply Disjoint_sym. eapply Disjoint_Included; [| | eapply Hdis' ].
+          eapply Included_trans; [| eapply bound_var_fun_map_get; eauto ]. now sets.
+          eapply Included_trans. eapply name_in_fundefs_bound_var_fundefs. sets.
         * sets.
       + eapply Disjoint_Included_r. eapply occurs_free_fun_map_remove_add_fundefs.
         eapply Union_Disjoint_r; [| now sets ].
-        eapply Union_Disjoint_r.
-        eapply Disjoint_Included_l.
-        eapply Included_trans; [| eapply fun_in_fundefs_bound_var_fundefs; eapply find_def_correct; eauto ].
-        now sets. eassumption. eapply find_def_correct. 
-        admit. (* easy *)
         eapply Disjoint_Included_l.
         now eapply bound_var_fun_map_get; eauto.
         eapply Disjoint_sym. eapply Disjoint_Included_l; [| eassumption ]. eapply Included_Union_compat.
@@ -1149,12 +1145,11 @@ Section Inline_correct.
         eapply Included_trans; [| eapply bound_var_fun_map_get; eauto ]. sets.
         eapply Included_trans. eapply name_in_fundefs_bound_var_fundefs. sets.
         sets.
-      + eapply Union_Disjoint_r. now sets. 
+      + (* eapply Union_Disjoint_r. now sets.  *)
         eapply Disjoint_Included_r. eapply image_apply_r_set_list. eassumption.
         eapply Union_Disjoint_r. now sets. xsets.
   Qed.
 
-  
   Lemma fun_map_vars_inv_remove S fm sig f :
     fun_map_vars fm S sig ->
     fun_map_vars (M.remove f fm) S sig.
@@ -1162,12 +1157,114 @@ Section Inline_correct.
     intros Hfm. intro; intros.
     destruct (peq f f0). subst. rewrite M.grs in H. inv H. rewrite M.gro in H; eauto.
     edestruct Hfm. eassumption. destructAll. repeat (split; [ now eauto |]).
-    split; [| split; [| split(* ; [| split ] *)]]; eauto.
+    split; [| split; [| split; [| split ]]]; eauto.
     - rewrite Dom_map_remove. sets.
     - sets. eapply Disjoint_Included_r. eapply occurs_free_fun_map_remove'. sets.
+    - sets. eapply Disjoint_Included_r. eapply bound_var_fun_map_remove'. sets.
     - rewrite Dom_map_remove. sets.
   Qed.
 
+
+  (* This invariant is used just for fundefs, instead of
+     [Disjoint _ (bound_var_fun_map fm) (bound_var_fundefs B :|: occurs_free_fundefs B)]
+     which does not hold after add_fundefs *)
+  
+  Definition just_for_fun_inv (B : fundefs) (fm : fun_map) :=
+    forall f ft xs e,
+      fun_in_fundefs B (f, ft, xs, e) ->
+      Disjoint _ (bound_var_fun_map (M.remove f fm)) (bound_var e :|: occurs_free e).
+
+  Lemma bound_var_fun_map_remove_set_same f v fm :
+    bound_var_fun_map (M.remove f (M.set f v fm)) \subset bound_var_fun_map fm.
+  Proof.
+    intros z Hin. inv Hin. destructAll. destruct (peq f x).
+    + subst. rewrite M.grs in H. congruence. 
+    + rewrite M.gro, M.gso in H; eauto. repeat eexists; eauto.
+  Qed. 
+
+  Lemma bound_var_fun_map_set f xs ft e fm :
+    bound_var_fun_map (M.set f (ft, xs, e) fm) \subset bound_var e :|: FromList xs :|: bound_var_fun_map fm.
+  Proof.
+    intros z Hin. inv Hin. destructAll. destruct (peq f x).
+    + subst. rewrite M.gss in H. inv H. eauto.
+    + rewrite M.gso in H; eauto. right. repeat eexists; eauto.
+  Qed. 
+  
+  Lemma bound_var_fun_map_remove_set_swap f g v fm :
+    f <> g ->
+    bound_var_fun_map (M.remove f (M.set g v fm)) <--> bound_var_fun_map (M.set g v (M.remove f fm)). 
+  Proof.
+    intros Hneq. split.
+    - intros z Hin. inv Hin. destructAll. destruct (peq f x).
+      + subst. rewrite M.grs in H. congruence. 
+      + rewrite remove_set_2 in H; eauto. repeat eexists; eauto.
+    - intros z Hin. inv Hin. destructAll. destruct (peq g x).
+      + subst. rewrite M.gss in H. inv H. repeat eexists; eauto.
+        rewrite M.gro. rewrite M.gss. reflexivity. eauto.
+      + rewrite M.gso in H; eauto.
+        destruct (peq f x).
+        * subst. rewrite M.grs in H. congruence. 
+        * rewrite M.gro in H; eauto. repeat eexists; eauto.
+          rewrite M.gro, M.gso; eauto.
+  Qed. 
+
+  
+  Lemma just_for_fun_inv_add_fundefs B fm :
+    unique_bindings_fundefs B ->
+    Disjoint _ (bound_var_fun_map fm) (bound_var_fundefs B :|: occurs_free_fundefs B) ->
+    Disjoint _ (bound_var_fundefs B) (occurs_free_fundefs B) -> 
+    just_for_fun_inv B (add_fundefs B fm).
+  Proof.
+    revert fm; induction B; intros fm Hun Hdis Hdis'.
+    - simpl. intro; intros. inv H.
+      + inv H0. inv Hun.
+        eapply Disjoint_Included_l.
+        eapply Included_trans.
+        now eapply bound_var_fun_map_remove_set_same.
+        now eapply bound_var_fun_map_add_fundefs_un; eauto.
+        eapply Union_Disjoint_l.
+        * eapply Union_Disjoint_r.
+          -- sets.
+          -- eapply Disjoint_Included_r. eapply occurs_free_in_fun with (B := Fcons f0 ft xs e0 B).
+             now left.  simpl.
+             repeat (eapply Union_Disjoint_r; [ now sets | ]).
+             rewrite bound_var_fundefs_Fcons in Hdis'. sets.
+        * eapply Disjoint_Included_r. eapply bound_var_occurs_free_Fcons_Included.
+          eassumption.
+      + inv Hun. assert (Hin := H0).
+        destruct (peq v f0); subst.
+        { exfalso. eapply fun_in_fundefs_bound_var_fundefs in Hin. eapply H6. eapply Hin. sets. }
+        
+        eapply IHB in H0.
+        * rewrite bound_var_fun_map_remove_set_swap; eauto.
+          eapply Disjoint_Included_l. 
+          eapply bound_var_fun_map_set. eapply Union_Disjoint_l; [| now sets ].
+          eapply Union_Disjoint_r.
+          -- eapply Disjoint_Included_r. eapply Included_trans; [| eapply fun_in_fundefs_bound_var_fundefs; eauto ]. now sets.
+             now sets.
+          -- eapply Disjoint_Included_r. eapply occurs_free_in_fun. eassumption. eapply Union_Disjoint_r; [| eapply Union_Disjoint_r ].
+             ++ eapply Disjoint_Included_r. eapply Included_trans; [| eapply fun_in_fundefs_bound_var_fundefs; eauto ]. now sets.
+                now sets.
+             ++ eapply Disjoint_Included_r. eapply name_in_fundefs_bound_var_fundefs. sets.
+             ++ rewrite bound_var_fundefs_Fcons, occurs_free_fundefs_Fcons in Hdis'.
+                eapply Disjoint_Included_r. eapply Included_Union_Setminus with (s2 := [set v]). now tci.
+                eapply Union_Disjoint_r. eapply Disjoint_Included; [| | eapply Hdis' ]; now xsets. now sets.
+        * eassumption.
+        * eapply Disjoint_Included_r; [| eassumption ].
+          normalize_bound_var. normalize_occurs_free. (* XXX make lemma pls *)
+          rewrite !Union_assoc.
+          rewrite Union_Setminus_Included with (s3 := [set v]); tci; sets.
+        * rewrite bound_var_fundefs_Fcons in Hdis'.
+          rewrite occurs_free_fundefs_Fcons in Hdis'.
+          eapply Disjoint_Included_r.
+          eapply Included_Union_Setminus_Included_Union with (s3 := [set v]); tci. reflexivity.
+          eapply Included_Union_preserv_l. reflexivity.
+          eapply Union_Disjoint_r.
+          eapply Disjoint_Included; [| | eapply Hdis' ]; sets.
+          sets.
+    - intro; intros. inv H.
+  Qed.
+    
   Opaque preord_exp'.
 
 
@@ -1195,17 +1292,15 @@ Section Inline_correct.
     | Ecase x l => exists cl, e' = Ecase (apply_r sig x) cl /\ Forall2 (fun p p' : ctor_tag * exp => fst p = fst p') l cl
     | _ => True
     end.
-             
-   
-  Lemma inline_correct_mut d (Hleq : (d <= G)%nat) : 
+
+    Lemma inline_correct_mut d (Hleq : (d <= G)%nat) : 
     (forall e sig fm st S str_flag 
             (Hun : unique_bindings e)
             (Hdis1 : Disjoint _ (bound_var e) (occurs_free e :|: occurs_free_fun_map fm))
-            (Hdis1' : Disjoint _ (bound_var e :|: bound_var_fun_map fm) (image (apply_r sig) (occurs_free e :|: occurs_free_fun_map fm)))
-            (Hdis2 : Disjoint _ S ((bound_var e :|: bound_var_fun_map fm) :|: image (apply_r sig) (occurs_free e :|: occurs_free_fun_map fm)))
-            (Hdis3 : Disjoint _ (bound_var e \\ funnames_in_exp e) (Dom_map fm))
-            (* (Hdis5 : Disjoint _ (bound_var_fun_map fm) (bound_var e :|: occurs_free e)) *)
-            (* (Hdis5 : Disjoint _ (bound_var_fun_map fm) (funnames_in_exp e)) *)
+            (Hdis2 : Disjoint _ (bound_var e :|: bound_var_fun_map fm) (image (apply_r sig) (occurs_free e :|: occurs_free_fun_map fm)))
+            (Hdis3 : Disjoint _ S ((bound_var e :|: bound_var_fun_map fm) :|: image (apply_r sig) (occurs_free e :|: occurs_free_fun_map fm)))
+            (Hdis4 : Disjoint _ (bound_var e) (Dom_map fm))
+            (Hdis5 : Disjoint _ (bound_var_fun_map fm) (bound_var e :|: occurs_free e))
             
             (Hfm : fun_map_vars fm S sig),
         {{ fun _ s => fresh S (next_var (fst s)) }}
@@ -1224,10 +1319,10 @@ Section Inline_correct.
     (forall B sig sig0 fm st S
             (Hun : unique_bindings_fundefs B)
             (Hdis1 : Disjoint _ (bound_var_fundefs B) (occurs_free_fundefs B :|: (occurs_free_fun_map fm \\ name_in_fundefs B)))
-            (Hdis1' : Disjoint _ (bound_var_fundefs B :|: bound_var_fun_map fm) (image (apply_r sig) (occurs_free_fundefs B :|: occurs_free_fun_map fm)))
-            (Hdis2 : Disjoint _ S ((bound_var_fundefs B :|: bound_var_fun_map fm):|: image (apply_r sig) (occurs_free_fundefs B :|: occurs_free_fun_map fm)))
-            (Hdis3 : Disjoint _ (bound_var_fundefs B \\ name_in_fundefs B \\ funnames_in_fundefs B) (Dom_map fm))
-            (* (Hdis5 : Disjoint _ (bound_var_fun_map fm) (bound_var_fundefs B :|: occurs_free_fundefs B)) *)
+            (Hdis2 : Disjoint _ (bound_var_fundefs B :|: bound_var_fun_map fm) (image (apply_r sig) (occurs_free_fundefs B :|: occurs_free_fun_map fm)))
+            (Hdis3 : Disjoint _ S ((bound_var_fundefs B :|: bound_var_fun_map fm):|: image (apply_r sig) (occurs_free_fundefs B :|: occurs_free_fun_map fm)))
+            (Hdis4 : Disjoint _ (bound_var_fundefs B \\ name_in_fundefs B) (Dom_map fm))
+            (Hdis5 : just_for_fun_inv B fm)
                         
             (Hfm : fun_map_vars fm S sig)
             (Hnames1 : NoDup (apply_r_list sig (all_fun_name B)))
@@ -1266,18 +1361,18 @@ Section Inline_correct.
         eapply Disjoint_Singleton_r. eassumption.
       + repeat normalize_bound_var_in_ctx. repeat normalize_occurs_free_in_ctx.
         eapply Disjoint_Included_r. eapply image_apply_r_set. eapply Union_Disjoint_r.
-        eapply Disjoint_sym. eapply Disjoint_Included; [| | eapply Hdis2 ]. now sets. now sets.
-        rewrite Setminus_Union_distr. eapply Disjoint_Included; [| | eapply Hdis1' ]. now sets. now sets.
+        eapply Disjoint_sym. eapply Disjoint_Included; [| | eapply Hdis3 ]. now sets. now sets.
+        rewrite Setminus_Union_distr. eapply Disjoint_Included; [| | eapply Hdis2 ]. now sets. now sets.
       + eapply Disjoint_Included_r.
         eapply Included_Union_compat. reflexivity.
         eapply image_apply_r_set. 
         repeat normalize_bound_var_in_ctx. repeat normalize_occurs_free_in_ctx.
         eapply Union_Disjoint_r. now sets.
         eapply Union_Disjoint_r. now sets.
-        eapply Disjoint_Included; [| | eapply Hdis2 ].
+        eapply Disjoint_Included; [| | eapply Hdis3 ].
         rewrite Setminus_Union_distr. rewrite !image_Union. now xsets. now sets.
       + eapply Disjoint_Included_l; [| eassumption ]. normalize_bound_var. sets.
-      (* + eapply Disjoint_Included_r. eapply bound_var_occurs_free_Econstr_Included. eassumption. *)
+      + eapply Disjoint_Included_r. eapply bound_var_occurs_free_Econstr_Included. eassumption.
       + eapply fun_map_vars_set. eassumption.
       + intros e' w2. eapply return_triple.
         intros _ st'. intros [Hf1 [Hf2 [Hf3 [Hf4 [Hun [Hsub [Hsub' [Hsh [Hstr Hsem]]]]]]]]].
@@ -1308,14 +1403,13 @@ Section Inline_correct.
              omega. normalize_occurs_free. sets.
           -- rewrite preord_val_eq. split. reflexivity.
              eapply Forall2_Forall2_asym_included. eassumption.
-          -- intros Hc. eapply Hdis2. constructor. eapply Hf'. eapply Hf1. 
+          -- intros Hc. eapply Hdis3. constructor. eapply Hf'. eapply Hf1. 
              right. normalize_occurs_free. eapply image_monotonic; [| eassumption ]. sets.
           -- eapply fun_map_inv_antimon. eapply fun_map_inv_set. eapply fun_map_inv_i_mon. eassumption. omega.
              intros Hc. inv Hc.
              ++ eapply Hdis1. normalize_bound_var. normalize_occurs_free. constructor. now right. eauto.
-             ++ admit. (* easy -- funnames_in_exp lemmas *)
-                (* eapply Hdis3. constructor. normalize_bound_var. simpl. now right. eassumption. *)
-             ++ intros Hc. eapply Hdis2. constructor; try eassumption. rewrite image_Union. do 2 right. eassumption.
+             ++ eapply Hdis4. constructor. normalize_bound_var. now right. eassumption.
+             ++ intros Hc. eapply Hdis3. constructor; try eassumption. rewrite image_Union. do 2 right. eassumption.
              ++ normalize_occurs_free. rewrite !Union_assoc. rewrite Union_Setminus_Included; sets; tci.
     - (* Ecase [] *)
       simpl. eapply bind_triple.
@@ -1336,16 +1430,12 @@ Section Inline_correct.
         * repeat normalize_bound_var_in_ctx. repeat normalize_occurs_free_in_ctx.
           eapply Disjoint_Included; [| | eapply Hdis1 ]; sets.
         * repeat normalize_bound_var_in_ctx. repeat normalize_occurs_free_in_ctx.
-          eapply Disjoint_Included; [| | eapply Hdis1' ]; sets.
+          eapply Disjoint_Included; [| | eapply Hdis2 ]; sets.
         * repeat normalize_bound_var_in_ctx. repeat normalize_occurs_free_in_ctx.
           xsets.
-        * repeat normalize_bound_var_in_ctx. repeat normalize_occurs_free_in_ctx.
-          admit. (* easy -- funnames_in_exp disjoint lemmas *)
-          (* eapply Disjoint_Included_l; [| eapply Hdis3 ]. rewrite Setminus_Union_distr. eapply Included_Union_preserv_l. *)
-          (* simpl. sets.  *)
-          (* simpl in Hdis3. now sets. *)
-        (* * eapply Disjoint_Included_r. eapply bound_var_occurs_free_Ecase_Included. 2:{ eassumption. } *)
-        (*   now left. *)
+        * repeat normalize_bound_var_in_ctx. repeat normalize_occurs_free_in_ctx. now sets.
+        * eapply Disjoint_Included_r. eapply bound_var_occurs_free_Ecase_Included. 2:{ eassumption. }
+          now left.
         * eassumption.
       + intros e' w. simpl.
         eapply pre_curry_l. intros Hf'. eapply pre_strenghtening.
@@ -1362,12 +1452,11 @@ Section Inline_correct.
           -- repeat normalize_bound_var_in_ctx. repeat normalize_occurs_free_in_ctx.
              eapply Disjoint_Included; [| | eapply Hdis1 ]; sets.
           -- repeat normalize_bound_var_in_ctx. repeat normalize_occurs_free_in_ctx.
-             eapply Disjoint_Included; [| | eapply Hdis1' ]; sets.
+             eapply Disjoint_Included; [| | eapply Hdis2 ]; sets.
           -- repeat normalize_bound_var_in_ctx. repeat normalize_occurs_free_in_ctx.
              xsets.
-          -- repeat normalize_bound_var_in_ctx. repeat normalize_occurs_free_in_ctx.
-             admit. (* easy -- disjoint lemmas *)
-          (* -- eapply Disjoint_Included_r. eapply bound_var_occurs_free_Ecase_cons_Included. eassumption. *)
+          -- repeat normalize_bound_var_in_ctx. repeat normalize_occurs_free_in_ctx. now sets.
+          -- eapply Disjoint_Included_r. eapply bound_var_occurs_free_Ecase_cons_Included. eassumption.
           -- eassumption.
         * intros ce w'. simpl. eapply pre_curry_l. intros Hbv. eapply pre_curry_l. intros Hleq1.
           eapply pre_curry_l. intros Hf''.
@@ -1414,18 +1503,18 @@ Section Inline_correct.
         eapply Disjoint_Singleton_r. eassumption.
       + repeat normalize_bound_var_in_ctx. repeat normalize_occurs_free_in_ctx.
         eapply Disjoint_Included_r. eapply image_apply_r_set. eapply Union_Disjoint_r.
-        eapply Disjoint_sym. eapply Disjoint_Included; [| | eapply Hdis2 ]. now sets. now sets.
-        rewrite Setminus_Union_distr. eapply Disjoint_Included; [| | eapply Hdis1' ]. now sets. now sets.  
+        eapply Disjoint_sym. eapply Disjoint_Included; [| | eapply Hdis3 ]. now sets. now sets.
+        rewrite Setminus_Union_distr. eapply Disjoint_Included; [| | eapply Hdis2 ]. now sets. now sets.  
       + eapply Disjoint_Included_r.
         eapply Included_Union_compat. reflexivity.
         eapply image_apply_r_set. 
         repeat normalize_bound_var_in_ctx. repeat normalize_occurs_free_in_ctx.
         eapply Union_Disjoint_r. now sets.
         eapply Union_Disjoint_r. now sets.
-        eapply Disjoint_Included; [| | eapply Hdis2 ].
+        eapply Disjoint_Included; [| | eapply Hdis3 ].
         rewrite Setminus_Union_distr. rewrite !image_Union. now xsets. now sets.
       + eapply Disjoint_Included_l; [| eassumption ]. normalize_bound_var. sets.
-      (* + eapply Disjoint_Included_r. eapply bound_var_occurs_free_Eproj_Included. eassumption. *)
+      + eapply Disjoint_Included_r. eapply bound_var_occurs_free_Eproj_Included. eassumption.
       + eapply fun_map_vars_set. eassumption.
       + intros e' w2. eapply return_triple.
         intros _ st'. intros [Hf1 [Hf2 [Hf3 [Hf4 [Hun [Hsub [Hsub' [Hsh [Hstr Hsem]]]]]]]]].
@@ -1453,15 +1542,13 @@ Section Inline_correct.
           -- eapply preord_env_P_inj_antimon. eapply preord_env_P_inj_monotonic; [| eassumption ].
              omega. normalize_occurs_free. sets.
           -- eassumption.
-          -- intros Hc. eapply Hdis2. constructor. eapply Hf'. eapply Hf1. 
+          -- intros Hc. eapply Hdis3. constructor. eapply Hf'. eapply Hf1. 
              right. normalize_occurs_free. eapply image_monotonic; [| eassumption ]. sets.
           -- eapply fun_map_inv_antimon. eapply fun_map_inv_set. eapply fun_map_inv_i_mon. eassumption. omega.
              intros Hc. inv Hc. 
              ++ eapply Hdis1. normalize_bound_var. constructor. now right. now right; eauto.
-             ++ admit. (* easy -- disjoint funnames_in_exp lemmas *)
-                (* eapply Hdis3. constructor. normalize_bound_var. simpl.                 *)
-                (* now right. eassumption.  *)
-             ++ intros Hc. eapply Hdis2. constructor; try eassumption. rewrite image_Union. do 2 right. eassumption.
+             ++ eapply Hdis4. constructor. normalize_bound_var. now right. eassumption. 
+             ++ intros Hc. eapply Hdis3. constructor; try eassumption. rewrite image_Union. do 2 right. eassumption.
              ++ normalize_occurs_free. rewrite !Union_assoc. rewrite Union_Setminus_Included; sets; tci.
     - (* Eletapp *)
       simpl. Opaque beta_contract.  destruct (update_letApp St IH f ft (apply_r_list sig ys) st) as [[s1 s2] b].
@@ -1479,17 +1566,17 @@ Section Inline_correct.
           rewrite Setminus_Union_distr. now sets. eapply Disjoint_Singleton_r. eassumption.
         - repeat normalize_bound_var_in_ctx. repeat normalize_occurs_free_in_ctx.
           eapply Disjoint_Included_r. eapply image_apply_r_set. eapply Union_Disjoint_r.
-          eapply Disjoint_sym. eapply Disjoint_Included; [| | eapply Hdis2 ]. now sets. now sets.
-          rewrite Setminus_Union_distr. eapply Disjoint_Included; [| | eapply Hdis1' ]. now sets. now sets.
+          eapply Disjoint_sym. eapply Disjoint_Included; [| | eapply Hdis3 ]. now sets. now sets.
+          rewrite Setminus_Union_distr. eapply Disjoint_Included; [| | eapply Hdis2 ]. now sets. now sets.
         - repeat normalize_bound_var_in_ctx. repeat normalize_occurs_free_in_ctx.
           eapply Disjoint_Included_r.
           eapply Included_Union_compat. reflexivity.
           eapply image_apply_r_set. 
           eapply Union_Disjoint_r. now sets. eapply Union_Disjoint_r. now sets.
-          eapply Disjoint_Included; [| | eapply Hdis2 ]; [| now sets ].
+          eapply Disjoint_Included; [| | eapply Hdis3 ]; [| now sets ].
           eapply Included_Union_preserv_r. eapply image_monotonic. rewrite Setminus_Union_distr. sets. 
         - eapply Disjoint_Included_l; [| eassumption ]. normalize_bound_var. sets.
-        (* - eapply Disjoint_Included_r. eapply bound_var_occurs_free_Eletapp_Included. eassumption. *)
+        - eapply Disjoint_Included_r. eapply bound_var_occurs_free_Eletapp_Included. eassumption.
         - eapply fun_map_vars_set. eassumption.
         - intros e' w2. eapply return_triple.
           intros _ st'. intros [Hf1 [Hf2 [Hf3 [Hf4 [Hun [Hsub [Hsub' [Hsh [Hstr Hsem]]]]]]]]].
@@ -1521,14 +1608,13 @@ Section Inline_correct.
             -- eapply preord_env_P_inj_antimon. eapply preord_env_P_inj_monotonic; [| eassumption ].
                omega. normalize_occurs_free. sets.
             -- eassumption.
-            -- intros Hc. eapply Hdis2. constructor. eapply Hf'. eapply Hf1. 
+            -- intros Hc. eapply Hdis3. constructor. eapply Hf'. eapply Hf1. 
                right. normalize_occurs_free. rewrite !image_Union. left. right. eassumption.
             -- eapply fun_map_inv_antimon. eapply fun_map_inv_set. eapply fun_map_inv_i_mon. eassumption. omega.
                intros Hc. inv Hc.
                ++ eapply Hdis1. constructor. normalize_bound_var. now right. right; eassumption.
-               ++ admit. (* easy -- disjoint funnames_in_exp lemmas *)
-                  (* eapply Hdis3. constructor. normalize_bound_var. now right. eassumption.  *)
-               ++ intros Hc. eapply Hdis2. constructor. eassumption. rewrite image_Union.
+               ++ eapply Hdis4. constructor. normalize_bound_var. now right. eassumption. 
+               ++ intros Hc. eapply Hdis3. constructor. eassumption. rewrite image_Union.
                   do 2 right. eassumption.
                ++ normalize_occurs_free. rewrite !Union_assoc. rewrite Union_Setminus_Included; sets; tci. }        
       destruct b. 
@@ -1545,16 +1631,16 @@ Section Inline_correct.
               + eapply le_trans. reflexivity.
                 eapply NPeano.Nat.div2_decr. omega.
               + eassumption.
-              + sets.
+              + eapply Union_Disjoint_r. clear H3. now sets. now sets.
               + eapply Disjoint_Included_r. eapply image_apply_r_set_list. unfold apply_r_list. rewrite map_length. eassumption.
                 eapply Union_Disjoint_r.
-                * eapply Disjoint_Included; [ | | eapply Hdis1' ].
+                * eapply Disjoint_Included; [ | | eapply Hdis2 ].
                   rewrite FromList_apply_list. normalize_occurs_free. rewrite !image_Union. now sets.
                   eapply Union_Included.
                   -- eapply Included_Union_preserv_r. 
                      eapply Included_trans; [| eapply bound_var_fun_map_get; eauto ]. sets.
                   -- eapply Included_trans. eapply bound_var_fun_map_remove. sets. 
-                * eapply Disjoint_Included; [| | eapply Hdis1' ]. rewrite image_Union.
+                * eapply Disjoint_Included; [| | eapply Hdis2 ]. rewrite image_Union.
                   eapply Included_Union_preserv_r. eapply image_monotonic. rewrite Setminus_Union_distr. 
                   eapply Union_Included.
                   -- eapply occurs_free_fun_map_get; eauto.
@@ -1564,22 +1650,21 @@ Section Inline_correct.
                      eapply Included_Union_preserv_r.
                      eapply Included_trans; [| eapply bound_var_fun_map_get; eauto ]. now sets.
               + repeat normalize_bound_var_in_ctx. repeat normalize_occurs_free_in_ctx. eapply Union_Disjoint_r.
-                eapply Union_Disjoint_r. now sets.
-                clear H7.
+                eapply Union_Disjoint_r. now sets. clear H8.
                 eapply Disjoint_Included_r. eapply bound_var_fun_map_remove. now sets.
                 eapply Disjoint_Included_r.
                 eapply image_apply_r_set_list. unfold apply_r_list. rewrite map_length. eassumption. 
                 eapply Union_Disjoint_r.
                 rewrite FromList_apply_list.
-                eapply Disjoint_Included; [| | eapply Hdis2 ]; [| now sets ]. rewrite !image_Union. now sets.
+                eapply Disjoint_Included; [| | eapply Hdis3 ]; [| now sets ]. rewrite !image_Union. now sets.
                 
                 rewrite !Setminus_Union_distr. rewrite image_Union. eapply Union_Disjoint_r.
-                eapply Disjoint_Included; [| | eapply H7 ]; now sets.
-                eapply Disjoint_Included; [| | eapply Hdis2 ].
+                eapply Disjoint_Included; [| | eapply H8 ]; now sets.
+                eapply Disjoint_Included; [| | eapply Hdis3 ].
                 eapply Included_trans. eapply image_monotonic. eapply Included_Setminus_compat.
                 eapply occurs_free_fun_map_remove. reflexivity. now sets. now sets.                
               + rewrite Dom_map_remove. sets.
-              (* + sets. *)
+              + sets.
               + eapply fun_map_vars_inv_remove.
                 intros ? ? ? ? ?.
                 edestruct Hfm; eauto. destructAll.
@@ -1587,7 +1672,7 @@ Section Inline_correct.
                 eapply Disjoint_Included_r. eapply image_apply_r_set_list.
                 unfold apply_r_list. rewrite list_length_map. eassumption.
                 eapply Union_Disjoint_r.
-                eapply Disjoint_Included; [| | eapply Hdis2 ]. normalize_occurs_free.
+                eapply Disjoint_Included; [| | eapply Hdis3 ]. normalize_occurs_free.
                 rewrite !image_Union. rewrite FromList_apply_list. now sets. now sets. now xsets.
             - intros ei w'. simpl. eapply pre_curry_l; intros Hfr. eapply pre_curry_l; intros Hleq1. 
               eapply pre_curry_l; intros Hfz.
@@ -1595,13 +1680,13 @@ Section Inline_correct.
               eapply pre_strenghtening.
               { intros. destructAll.
                 assert (Hfr' : fresh (S \\ [set z] \\ bound_var ei) (next_var (fst s))).
-                { intros u Hleq'. constructor. eapply H8; eauto.
-                  intros Hnin. eapply H12 in Hnin. unfold Ensembles.In, Range in Hnin. zify. omega. }
+                { intros u Hleq'. constructor. eapply H9; eauto.
+                  intros Hnin. eapply H13 in Hnin. unfold Ensembles.In, Range in Hnin. zify. omega. }
                 assert (Hbv : bound_var ei \subset S \\ [set z]).
                 { eapply Included_trans. eassumption. intros y Hin. unfold Ensembles.In, Range in *. inv Hin.
                   eapply Hfz. eassumption. }
                 
-                eapply (conj Hbv (conj H15 (conj H14 (conj H13 (conj H11 (conj H10 (conj H8 (conj H9 (conj H12 Hfr'))))))))). }
+                eapply (conj Hbv (conj H16 (conj H15 (conj H14 (conj H12 (conj H11 (conj H9 (conj H10 (conj H13 Hfr'))))))))). }
               
               eapply pre_curry_l. intros Hbv. eapply pre_curry_l. intros Hrel.
               eapply pre_curry_l. intros Hstr. eapply pre_curry_l. intros Hcase. eapply pre_curry_l. intros Hfv. eapply pre_curry_l. intros Hun.
@@ -1611,91 +1696,90 @@ Section Inline_correct.
                 - subst. eapply Union_Disjoint_l. now sets. eapply Disjoint_sym.
                   eapply Disjoint_Included_l. eapply Singleton_Included. eapply HSin.
                   repeat normalize_bound_var_in_ctx. repeat normalize_occurs_free_in_ctx.
-                  eapply Disjoint_Included_r; [ | eapply Hdis2 ]. now sets. 
+                  eapply Disjoint_Included_r; [ | eapply Hdis3 ]. now sets. 
                 - repeat normalize_bound_var_in_ctx. repeat normalize_occurs_free_in_ctx.
-                  inv H8.
+                  inv H9.
                   + eapply Disjoint_Included_r. eapply Singleton_Included. eassumption. eapply Union_Disjoint_l.
                     * sets.
                     * eapply Disjoint_Included_r. eassumption. eapply Disjoint_sym.
-                      eapply Disjoint_Included; [ | | eapply Hdis2 ]. now sets. now sets.
+                      eapply Disjoint_Included; [ | | eapply Hdis3 ]. now sets. now sets.
                   + eapply Disjoint_Included_r. eapply Included_trans. eapply Singleton_Included. eassumption.
                     eassumption.
                     eapply Disjoint_Included_r. eapply image_apply_r_set_list. unfold apply_r_list. rewrite map_length. now eauto.
                     rewrite !Setminus_Union_distr, image_Union.
                     eapply Union_Disjoint_r; [| eapply Union_Disjoint_r ].
                     rewrite FromList_apply_list.
-                    eapply Union_Disjoint_l. eapply Disjoint_Included; [| | eapply Hdis2 ]; now sets.
-                    eapply Disjoint_Included; [| | eapply Hdis1' ]; now sets.
+                    eapply Union_Disjoint_l. eapply Disjoint_Included; [| | eapply Hdis3 ]; now sets.
+                    eapply Disjoint_Included; [| | eapply Hdis2 ]; now sets.
                     eapply Union_Disjoint_l. now sets.
-                    eapply Disjoint_Included; [| | eapply Hdis1' ]. rewrite image_Union. eapply Included_Union_preserv_r.
+                    eapply Disjoint_Included; [| | eapply Hdis2 ]. rewrite image_Union. eapply Included_Union_preserv_r.
                     eapply image_monotonic. eapply occurs_free_fun_map_get; eauto. now sets. 
-                    eapply Union_Disjoint_l.  eapply Disjoint_Included; [| | eapply Hdis2 ]; try now sets.
+                    eapply Union_Disjoint_l.  eapply Disjoint_Included; [| | eapply Hdis3 ]; try now sets.
                     eapply Included_trans. eapply image_monotonic. eapply Included_Setminus_compat.
                     eapply occurs_free_fun_map_remove. reflexivity. now sets. 
-                    eapply Disjoint_Included; [| | eapply Hdis1' ]; try now sets.
+                    eapply Disjoint_Included; [| | eapply Hdis2 ]; try now sets.
                     eapply Included_trans. eapply image_monotonic. eapply Included_Setminus_compat.
                     eapply occurs_free_fun_map_remove. reflexivity. now sets. }
 
               
               eapply bind_triple.
-              + set (Q := fun s => fresh (S \\ [set z]) (next_var s) /\
-                                   next_var (fst w') <= next_var s /\
-                                   bound_var ei \subset
-                                             Range (next_var (fst w')) (next_var s) /\
-                                   fresh (S \\ [set z] \\ bound_var ei) (next_var s)). 
-                eapply click_spec with (P := Q).                                
-              + intros _u w''. eapply bind_triple.
-                * do 3 eapply frame_rule.
-                  { eapply IHd.
-                    + destruct d. simpl. omega.
-                      replace (Datatypes.S (Datatypes.S d)) with (Datatypes.S d + 1)%nat by omega. 
-                      eapply plus_lt_le_compat.
-                      eapply NPeano.Nat.lt_div2. omega.     
-                      destruct ((Nat.odd (Datatypes.S d))); simpl; omega.
-                    + eapply le_trans; [| eassumption ].
-                      assert (Heq := split_fuel_add d). rewrite Heq at 3. unfold split_fuel. simpl. omega.
-                    + eassumption.
-                    + repeat normalize_bound_var_in_ctx. repeat normalize_occurs_free_in_ctx.
-                      eapply Disjoint_Included_r. eapply Included_Union_Setminus with (s4 := [set x]). tci.
-                      eapply Union_Disjoint_r. rewrite Setminus_Union_distr. now eapply Disjoint_Included; [| | eapply Hdis1 ]; sets.
-                      eapply Disjoint_Singleton_r. eassumption.
-                    + repeat normalize_bound_var_in_ctx. repeat normalize_occurs_free_in_ctx.
-                      eapply Disjoint_Included_r.
-                      eapply image_apply_r_set. eapply Union_Disjoint_r. now sets.
-                      eapply Disjoint_Included; [| | eapply Hdis1' ]. rewrite Setminus_Union_distr. now sets. now sets.
-                    + repeat normalize_bound_var_in_ctx. repeat normalize_occurs_free_in_ctx.
-                      eapply Union_Disjoint_r. eapply Disjoint_Included; [| | eapply Hdis2 ]; now sets.
-                      eapply Disjoint_Included_r.
-                      eapply image_apply_r_set. eapply Union_Disjoint_r. now sets.
-                      eapply Disjoint_Included; [| | eapply Hdis2 ]. rewrite Setminus_Union_distr. now sets. now sets.
-                    + repeat normalize_bound_var_in_ctx. repeat normalize_occurs_free_in_ctx.
-                      eapply Disjoint_Included_l; [| eapply Hdis3 ]. simpl. sets.
-                    (* + eapply Disjoint_Included_r. eapply bound_var_occurs_free_Eletapp_Included. eassumption. *)
-                    + (* Make lemma if needed about fun_map_vars fm S (set_list (combine xs (apply_r_list sig l)) sig) *)
-                      intros ? ? ? ? ?. edestruct Hfm; eauto. destructAll.
-                      repeat (split; [ now eauto |]). eapply Union_Disjoint_r. now sets.
-                      eapply Disjoint_Included_r. eapply image_apply_r_set.
-                      eapply Union_Disjoint_r. now sets. now xsets. }
-                * { intros e' w'''. eapply return_triple. intros _ w'''' Hyp. destructAll.
-                    split; [| split; [| split; [| split; [| split; [| split; [| split ]]]]]].
-                    * eapply fresh_monotonic; [| eassumption ]. sets.
-                    * zify; omega.
-                    * eapply (proj1 (ub_app_ctx_f e')). split; [| split ]; [| eassumption |].
-                      eapply unique_bindings_inline_letapp; [ eassumption | | eassumption ].
-                      intros Hc. eapply H10 in Hc.
-                      unfold Ensembles.In, Range in Hc, Hfr. zify; omega.
-                      eapply Disjoint_Included_l. eapply bound_var_inline_letapp. eassumption.
-                      eapply Union_Disjoint_l.
-                      -- eapply Disjoint_Included_r. eassumption. eapply Disjoint_Singleton_l.
-                         intros Hc. unfold Ensembles.In, Range in Hc, Hfr. zify; omega.
-                      -- eapply Disjoint_Included. eassumption. eassumption.
-                         eapply Disjoint_Range. reflexivity.
-                    * eapply Included_trans. eapply occurs_fee_inline_letapp. eassumption.
-                      assert (Hsub : occurs_free ei :|: (occurs_free e' \\ stemctx.bound_stem_ctx C) \subset
-                                                 occurs_free ei :|: (occurs_free e' \\ [set r])).
-                      { edestruct inline_letapp_var_eq_alt. eassumption. inv H19; subst. now sets.
-                        inv H19. now sets. rewrite Union_Setminus_Included with (s5 := [set r]); tci. sets.
-                        sets. }
+              eapply click_spec with (P := fun s => fresh (S \\ [set z]) (next_var s) /\
+                                                    next_var (fst w') <= next_var s /\
+                                                    bound_var ei \subset Range (next_var (fst w')) (next_var s) /\
+                                                    fresh (S \\ [set z] \\ bound_var ei) (next_var s)).
+              intros _u w''. simpl. 
+              eapply bind_triple. 
+              + do 3 eapply frame_rule.
+                { eapply IHd.
+                  + destruct d. simpl. omega.
+                    replace (Datatypes.S (Datatypes.S d)) with (Datatypes.S d + 1)%nat by omega. 
+                    eapply plus_lt_le_compat.
+                    eapply NPeano.Nat.lt_div2. omega.     
+                    destruct ((Nat.odd (Datatypes.S d))); simpl; omega.
+                  + eapply le_trans; [| eassumption ].
+                    assert (Heq := split_fuel_add d). rewrite Heq at 3. unfold split_fuel. simpl. omega.
+                  + eassumption.
+                  + repeat normalize_bound_var_in_ctx. repeat normalize_occurs_free_in_ctx.
+                    eapply Disjoint_Included_r. eapply Included_Union_Setminus with (s4 := [set x]). tci.
+                    eapply Union_Disjoint_r. rewrite Setminus_Union_distr. now eapply Disjoint_Included; [| | eapply Hdis1 ]; sets.
+                    eapply Disjoint_Singleton_r. eassumption.
+                  + repeat normalize_bound_var_in_ctx. repeat normalize_occurs_free_in_ctx.
+                    eapply Disjoint_Included_r.
+                    eapply image_apply_r_set. eapply Union_Disjoint_r. now sets.
+                    eapply Disjoint_Included; [| | eapply Hdis2 ]. rewrite Setminus_Union_distr. now sets. now sets.
+                  + repeat normalize_bound_var_in_ctx. repeat normalize_occurs_free_in_ctx.
+                    eapply Union_Disjoint_r. eapply Disjoint_Included; [| | eapply Hdis3 ]; now sets.
+                    eapply Disjoint_Included_r.
+                    eapply image_apply_r_set. eapply Union_Disjoint_r. now sets.
+                    eapply Disjoint_Included; [| | eapply Hdis3 ]. rewrite Setminus_Union_distr. now sets. now sets.
+                  + repeat normalize_bound_var_in_ctx. repeat normalize_occurs_free_in_ctx.
+                    eapply Disjoint_Included_l; [| eapply Hdis4 ]. simpl. sets.
+                  + eapply Disjoint_Included_r. eapply bound_var_occurs_free_Eletapp_Included. eassumption.
+                  + (* Make lemma if needed about fun_map_vars fm S (set_list (combine xs (apply_r_list sig l)) sig) *)
+                    intros ? ? ? ? ?. edestruct Hfm; eauto. destructAll.
+                    repeat (split; [ now eauto |]). eapply Union_Disjoint_r. now sets.
+                    eapply Disjoint_Included_r. eapply image_apply_r_set.
+                    eapply Union_Disjoint_r. now sets. now xsets. }
+              + intros e' w'''. eapply return_triple. intros _ w'''' Hyp. destructAll.
+                split; [| split; [| split; [| split; [| split; [| split; [| split ]]]]]].
+                * eapply fresh_monotonic; [| eassumption ]. sets.
+                * zify; omega.
+                * eapply (proj1 (ub_app_ctx_f e')). split; [| split ]; [| eassumption |].
+                  eapply unique_bindings_inline_letapp; [ eassumption | | eassumption ].
+                  intros Hc. eapply H11 in Hc.
+                  unfold Ensembles.In, Range in Hc, Hfr. zify; omega.
+                  eapply Disjoint_Included_l. eapply bound_var_inline_letapp. eassumption.
+                  eapply Union_Disjoint_l.
+                  -- eapply Disjoint_Included_r. eassumption. eapply Disjoint_Singleton_l.
+                     intros Hc. unfold Ensembles.In, Range in Hc, Hfr. zify; omega.
+                  -- eapply Disjoint_Included. eassumption. eassumption.
+                     eapply Disjoint_Range. reflexivity.
+                * eapply Included_trans. eapply occurs_fee_inline_letapp. eassumption.
+                  assert (Hsub : occurs_free ei :|: (occurs_free e' \\ stemctx.bound_stem_ctx C) \subset
+                                             occurs_free ei :|: (occurs_free e' \\ [set r])).
+                  { edestruct inline_letapp_var_eq_alt. eassumption. inv H20; subst. now sets.
+                    inv H20. now sets. rewrite Union_Setminus_Included with (s5 := [set r]); tci. sets.
+                    sets. }
                   eapply Included_trans. eassumption. eapply Union_Included.
                   -- eapply Included_trans. eassumption. eapply Included_trans.
                      eapply image_apply_r_set_list. unfold apply_r_list. rewrite map_length. eassumption.
@@ -1716,18 +1800,18 @@ Section Inline_correct.
                      eapply Included_trans. eassumption. eapply Range_Subset. zify; omega. zify; omega.
                   -- eapply Included_trans. eassumption. eapply Range_Subset. zify; omega. zify; omega.
                 * eauto.
-                * intros Heq Hs; eauto. eapply straight_code_ctx_app. eassumption. eapply H17; eauto.
+                * intros Heq Hs; eauto. eapply straight_code_ctx_app. eassumption. eapply H18; eauto.
                 * intros. assert (Hadd := split_fuel_add d).
                   unfold split_fuel in *. simpl in Hadd. rewrite Hadd.
                   eapply inline_letapp_correct_alt with (C' := Hole_c);
-                    [ | | | | | | | |  now eauto | eassumption ]. 
+                            [ | | | | | | | |  now eauto | eassumption ]. 
                   -- eapply HEletapp.
                   -- eapply Eletapp_OOT.
                   -- eapply HProp.
                      eapply le_trans; [| eassumption ]. rewrite Hadd at 4. simpl. omega. 
-                  -- simpl. intros. edestruct H20 with (f0 := f). constructor. now left. eassumption. eassumption.
+                  -- simpl. intros. edestruct H21 with (f0 := f). constructor. now left. eassumption. eassumption.
                      destructAll. do 2 subst_exp. eapply Hrel.
-                     ++ edestruct preord_env_P_inj_get_list_l. now eapply H19. normalize_occurs_free. now sets.
+                     ++ edestruct preord_env_P_inj_get_list_l. now eapply H20. normalize_occurs_free. now sets.
                         eassumption. destructAll.                           
                         eapply preord_env_P_inj_set_lists_l'; try eassumption.
                         eapply preord_env_P_inj_monotonic; [| eassumption ]. omega.
@@ -1736,13 +1820,12 @@ Section Inline_correct.
                      ++ eapply fun_map_inv_antimon. eapply fun_map_inv_set_lists; [ | | | eassumption ].
                         ** eapply fun_map_inv_sig_extend_Disjoint. rewrite <- fun_map_inv_eq in *.
                            eapply fun_map_inv_i_mon. eapply fun_map_inv_remove.
-                           eapply fun_map_inv_mon. eassumption. omega. omega. sets. 
+                           eapply fun_map_inv_mon. eassumption. omega. omega. sets.
                         ** eassumption.
-                        ** eapply Union_Disjoint_r. sets.
-                           rewrite Dom_map_remove. sets.                        
+                        ** eapply Union_Disjoint_r. now sets. rewrite Dom_map_remove. sets. 
                         ** rewrite Union_Setminus_Included. sets. tci. sets. 
-                  -- intros. edestruct H20 with (f0 := f). constructor. now left. eassumption. eassumption.
-                     destructAll. subst_exp. eapply H18.
+                  -- intros. edestruct H21 with (f0 := f). constructor. now left. eassumption. eassumption.
+                     destructAll. subst_exp. eapply H19.
                      ++ rewrite apply_r_set_f_eq. eassumption.
                      ++ eapply fun_map_inv_antimon.
                         2:{ eapply Included_trans. eapply Included_Union_Setminus with (s4 := [set x]); tci.
@@ -1755,28 +1838,27 @@ Section Inline_correct.
                            eapply eq_env_P_refl. 
                            eapply eq_env_P_antimon. eassumption.
                            normalize_bound_var_ctx. normalize_sets. intros y Hin Hin'.
-                           eapply bound_var_inline_letapp in Hin'; [| eassumption ]. eapply Hdis2.
+                           eapply bound_var_inline_letapp in Hin'; [| eassumption ]. eapply Hdis3.
                            constructor. 2:{ right. rewrite image_Union. right. eassumption. }
-                           inv Hin'. inv H29.
+                           inv Hin'. inv H30.
                            eapply Hfx. unfold Ensembles.In, Range in *. zify; omega.
-                           eapply H10 in H29. eapply Hfx. unfold Ensembles.In, Range in *. zify; omega.
+                           eapply H11 in H30. eapply Hfx. unfold Ensembles.In, Range in *. zify; omega.
                         ** eassumption.
-                        ** admit. (* eassy Disjoint funnames_in_exp lemmas *)
-                        (* intros Hc. eapply Hdis3. constructor. 2:{ eassumption. } now eauto. *)
+                        ** intros Hc. eapply Hdis4. constructor. 2:{ eassumption. } now eauto.
                         ** intros Hc. eapply Hdis1. constructor. now constructor. now eauto.
                         ** intros Hc. inv Hc; eauto.
                   -- eassumption.
                   -- normalize_bound_var_ctx. normalize_sets.
                      eapply Disjoint_Included_l. eapply bound_var_inline_letapp. eassumption.
-                     eapply Disjoint_Included; [| | eapply Hdis2 ]. normalize_occurs_free. rewrite image_Union. now sets.
+                     eapply Disjoint_Included; [| | eapply Hdis3 ]. normalize_occurs_free. rewrite image_Union. now sets.
                      eapply Union_Included. intros u Hc. inv Hc. eapply Hfx. unfold Ensembles.In, Range in *. zify; omega.
-                     intros u Hc. eapply H10 in Hc. unfold Ensembles.In, Range in *. eapply Hfx. zify; omega.
-                  -- intros Hc. eapply Hdis1'. normalize_occurs_free. normalize_bound_var.
-                     constructor. now eauto. rewrite !image_Union. now eauto. }
-              + eapply post_weakening. 
+                     intros u Hc. eapply H11 in Hc. unfold Ensembles.In, Range in *. eapply Hfx. zify; omega.
+                  -- intros Hc. eapply Hdis2. normalize_occurs_free. normalize_bound_var.
+                     constructor. now eauto. rewrite !image_Union. now eauto.
+             + eapply post_weakening. 
                 2:{ eapply pre_transfer_r. eapply pre_strenghtening. 2:{
                       eapply post_weakening; [| eassumption ]. simpl. intros.
-                      eapply (conj H8 H9). }
+                      eapply (conj H9 H10). }
                     simpl. intros.  destructAll. eapply fresh_monotonic; [| eassumption ]. sets. }
                 simpl. intros. destructAll.
                 split; [| split; [| split; [| split; [| split ]]]]; eauto.
@@ -1790,14 +1872,13 @@ Section Inline_correct.
       eapply bind_triple. eapply pre_transfer_r. now eapply get_fresh_names_spec. intros xs w. simpl.
       eapply pre_curry_l. intros Hf'. eapply pre_curry_l. intros Hnd.  eapply pre_curry_l. intros Hlen.
       
-      (* assert (Hfm' : fun_map_vars (add_fundefs f2 fm) (S \\ FromList xs) (set_list (combine (all_fun_name f2) xs) sig)). *)
-      (* { eapply fun_map_vars_def_funs; (try now eauto). *)
-      (*   + repeat normalize_bound_var_in_ctx. repeat normalize_occurs_free_in_ctx. *)
-      (*     eapply Disjoint_Included; [| | eapply Hdis1 ]; sets. *)
-      (*   + repeat normalize_bound_var_in_ctx. repeat normalize_occurs_free_in_ctx. sets. *)
-          
-      (*   + repeat normalize_bound_var_in_ctx. repeat normalize_occurs_free_in_ctx. sets. *)
-      (*   + repeat normalize_bound_var_in_ctx. repeat normalize_occurs_free_in_ctx. xsets. } *)
+      assert (Hfm' : fun_map_vars (add_fundefs f2 fm) (S \\ FromList xs) (set_list (combine (all_fun_name f2) xs) sig)).
+      { eapply fun_map_vars_def_funs; (try now eauto).
+        + repeat normalize_bound_var_in_ctx. repeat normalize_occurs_free_in_ctx.
+          eapply Disjoint_Included; [| | eapply Hdis1 ]; sets.
+        + repeat normalize_bound_var_in_ctx. repeat normalize_occurs_free_in_ctx. sets.
+        + repeat normalize_bound_var_in_ctx. repeat normalize_occurs_free_in_ctx. sets.
+        + repeat normalize_bound_var_in_ctx. repeat normalize_occurs_free_in_ctx. xsets. }
 
       assert (Hnd' := NoDup_all_fun_name _ H2).
       assert (Hseq :  apply_r_list (set_list (combine (all_fun_name f2) xs) sig) (all_fun_name f2) = xs).
@@ -1808,37 +1889,45 @@ Section Inline_correct.
         - eassumption.
         - repeat normalize_occurs_free_in_ctx. repeat normalize_bound_var_in_ctx. eapply Union_Disjoint_r.
           eapply Disjoint_Included; [| | eapply Hdis1 ]; now sets.
-          admit. (* easy *) 
-          (* eapply Disjoint_Included; [| | eapply Hdis1 ]; now sets. *)
+          eapply Disjoint_Included_r.
+          eapply Included_Setminus_compat. now eapply occurs_free_fun_map_add_fundefs. reflexivity.
+          rewrite !Setminus_Union_distr. rewrite Setminus_Same_set_Empty_set. normalize_sets.
+          eapply Disjoint_Included; [| | eapply Hdis1 ]; now sets.
         - eapply Disjoint_Included_r.
           + eapply Included_trans. eapply image_apply_r_set_list. now eauto.
             rewrite <- Same_set_all_fun_name. rewrite !Setminus_Union_distr. eapply Included_Union_compat. reflexivity.
             reflexivity.
-          + admit. (* I think OK *)
-            (* eapply Union_Disjoint_r. *)
-            (* * eapply Disjoint_sym. eapply Disjoint_Included; [| | eapply Hdis2 ]. normalize_bound_var. now sets. eassumption. *)
-            (* * eapply Disjoint_Included; [| | eapply Hdis1' ]. normalize_occurs_free. eapply image_monotonic. now sets. *)
-            (*   normalize_bound_var. now sets. *)
-        - admit.
-          (* repeat normalize_occurs_free_in_ctx. repeat normalize_bound_var_in_ctx. eapply Union_Disjoint_r. *)
-          (* + sets. *)
-          (* + eapply Disjoint_Included_r. eapply image_apply_r_set_list. now eauto. *)
-          (*   rewrite <- Same_set_all_fun_name. rewrite !Setminus_Union_distr. rewrite !image_Union.  *)
-          (*   repeat (eapply Union_Disjoint_r; sets). *)
-          (*   now xsets. *)
-          (*   now xsets. *)
+          + eapply Union_Disjoint_r.
+            * eapply Disjoint_sym. eapply Disjoint_Included; [| | eapply Hdis3 ].
+              normalize_bound_var. eapply Union_Included. sets.
+              eapply Included_trans. eapply bound_var_fun_map_add_fundefs_un. eassumption. sets.
+              eassumption.
+            * eapply Disjoint_Included; [| | eapply Hdis2 ]. normalize_occurs_free. eapply image_monotonic.
+              eapply Union_Included. sets. eapply Included_trans. eapply Included_Setminus_compat.
+              eapply occurs_free_fun_map_add_fundefs. reflexivity. rewrite !Setminus_Union_distr. now sets.
+              normalize_bound_var. eapply Union_Included. now sets.
+              eapply Included_trans. eapply bound_var_fun_map_add_fundefs_un. eassumption. sets.
+        - repeat normalize_occurs_free_in_ctx. repeat normalize_bound_var_in_ctx. eapply Union_Disjoint_r. eapply Union_Disjoint_r. 
+          + sets.
+          + eapply Disjoint_Included_r. eapply bound_var_fun_map_add_fundefs_un. eassumption.
+            eapply Disjoint_Included; [| | eapply Hdis3 ]; sets.
+          + eapply Disjoint_Included_r. eapply image_apply_r_set_list. now eauto.
+            rewrite <- Same_set_all_fun_name. rewrite !Setminus_Union_distr. rewrite !image_Union. 
+            repeat (eapply Union_Disjoint_r; sets).
+            now xsets.
+            eapply Disjoint_Included_r. eapply image_monotonic.
+            eapply Included_Setminus_compat. eapply occurs_free_fun_map_add_fundefs. reflexivity. xsets. 
         - repeat normalize_occurs_free_in_ctx. repeat normalize_bound_var_in_ctx.
-          simpl in *. rewrite Setminus_Union_distr, <- Setminus_Union in Hdis3.
-          rewrite Dom_map_add_fundefs. 
-          admit. (* more lemmas about funnames_in_exp *)
-        - repeat normalize_occurs_free_in_ctx. repeat normalize_bound_var_in_ctx. sets. admit.
-        (* - eapply fun_map_vars_set_list. 3:{ eassumption. }  admit. *)
-        (* eassumption. *)
+          eapply Disjoint_Included_r. eapply Dom_map_add_fundefs. sets.
+        - repeat normalize_occurs_free_in_ctx. repeat normalize_bound_var_in_ctx.
+          eapply just_for_fun_inv_add_fundefs. eassumption. sets.
+          eapply Disjoint_Included; [| | eapply Hdis1 ]; sets.
+        - eassumption.
         - rewrite Hseq. eassumption.
         - rewrite Hseq. eapply Union_Disjoint_l. now sets.
-          eapply Disjoint_Included_r. eassumption. eapply Disjoint_sym. eapply Disjoint_Included_r; [| eapply Hdis2 ]. normalize_bound_var.
-          eapply Union_Included. now sets. eapply Included_trans. eapply bound_var_fun_map_add_fundefs_un. eassumption.
-          sets. } 
+          eapply Disjoint_Included_r. eassumption. eapply Disjoint_sym. eapply Disjoint_Included_r; [| eapply Hdis3 ]. normalize_bound_var.
+          eapply Union_Included. now sets.
+          eapply Included_trans. eapply bound_var_fun_map_add_fundefs_un. eassumption. sets. } 
       
       intros fds' w'. simpl.
       eapply pre_curry_l. intros Hsub. eapply pre_curry_l. intros Hr. 
@@ -1857,14 +1946,14 @@ Section Inline_correct.
               eapply Disjoint_Included_l. eapply Included_Union_compat. reflexivity. eapply bound_var_fun_map_add_fundefs_un. eassumption. 
               eapply Disjoint_Included_r. 
               eapply image_apply_r_set_list. now eauto. eapply Union_Disjoint_r.
-              * eapply Disjoint_sym. eapply Disjoint_Included; [| | eapply Hdis2 ]. now sets. eassumption.
+              * eapply Disjoint_sym. eapply Disjoint_Included; [| | eapply Hdis3 ]. now sets. eassumption.
               * rewrite <- Same_set_all_fun_name. rewrite Setminus_Union_distr.
                 rewrite image_Union. eapply Union_Disjoint_r.
-                eapply Disjoint_Included; [| | eapply Hdis1' ]. now sets. now sets.
+                eapply Disjoint_Included; [| | eapply Hdis2 ]. now sets. now sets.
                 eapply Disjoint_Included_r. eapply image_monotonic. eapply Included_Setminus_compat.
                 eapply occurs_free_fun_map_add_fundefs. reflexivity.
                 rewrite !Setminus_Union_distr. rewrite !Setminus_Same_set_Empty_set. repeat normalize_sets.
-                eapply Disjoint_Included; [| | eapply Hdis1' ]. now sets. now sets.
+                eapply Disjoint_Included; [| | eapply Hdis2 ]. now sets. now sets.
             + repeat normalize_bound_var_in_ctx. repeat normalize_occurs_free_in_ctx. eapply Union_Disjoint_r. eapply Union_Disjoint_r. 
               now sets.
               eapply Disjoint_Included_r. eapply bound_var_fun_map_add_fundefs_un. eassumption. now xsets.
@@ -1873,29 +1962,29 @@ Section Inline_correct.
               * now sets.
               * rewrite <- Same_set_all_fun_name. rewrite Setminus_Union_distr.
                 rewrite image_Union. eapply Union_Disjoint_r.
-                eapply Disjoint_Included; [| | eapply Hdis2 ]. now sets. now sets.
+                eapply Disjoint_Included; [| | eapply Hdis3 ]. now sets. now sets.
                 eapply Disjoint_Included_r. eapply image_monotonic. eapply Included_Setminus_compat.
                 eapply occurs_free_fun_map_add_fundefs. reflexivity.
                 rewrite !Setminus_Union_distr. rewrite !Setminus_Same_set_Empty_set. repeat normalize_sets.
-                eapply Disjoint_Included; [| | eapply Hdis2 ]. now sets. now sets.
+                eapply Disjoint_Included; [| | eapply Hdis3 ]. now sets. now sets.
             + repeat normalize_bound_var_in_ctx. repeat normalize_occurs_free_in_ctx.
               rewrite Dom_map_add_fundefs. eapply Union_Disjoint_r.
               * eapply Disjoint_Included_r. eapply name_in_fundefs_bound_var_fundefs. now sets.
-              * admit. (* more lemmas about funnames_in_exp *)
-            (* + repeat normalize_bound_var_in_ctx. repeat normalize_occurs_free_in_ctx. *)
-            (*   eapply Disjoint_Included_l. *)
-            (*   * eapply bound_var_fun_map_add_fundefs_un. eassumption. *)
-            (*   * eapply Union_Disjoint_l. *)
-            (*     -- eapply Union_Disjoint_r. now sets. *)
-            (*        eapply Disjoint_Included_r. *)
-            (*        eapply Included_Union_Setminus with (s2 := name_in_fundefs f2). tci. *)
-            (*        eapply Union_Disjoint_r; [| now sets ]. *)
-            (*        eapply Disjoint_Included; [| | eapply Hdis1 ]; now sets. *)
-            (*     -- eapply Union_Disjoint_r. now sets. *)
-            (*        eapply Disjoint_Included; [| | eapply Hdis5 ]; [| now sets ]. *)
-            (*        rewrite !Union_assoc. rewrite Union_commut. rewrite <- Union_Included_Union_Setminus. *)
-            (*        now sets. now tci.  eapply Included_trans. eapply name_in_fundefs_bound_var_fundefs. now sets. *)
-            + admit. (* fun_map_vars lemma *) }
+              * sets.
+            + repeat normalize_bound_var_in_ctx. repeat normalize_occurs_free_in_ctx.
+              eapply Disjoint_Included_l.
+              * eapply bound_var_fun_map_add_fundefs_un. eassumption.
+              * eapply Union_Disjoint_l.
+                -- eapply Union_Disjoint_r. now sets.
+                   eapply Disjoint_Included_r.
+                   eapply Included_Union_Setminus with (s2 := name_in_fundefs f2). tci.
+                   eapply Union_Disjoint_r; [| now sets ].
+                   eapply Disjoint_Included; [| | eapply Hdis1 ]; now sets.
+                -- eapply Union_Disjoint_r. now sets.
+                   eapply Disjoint_Included; [| | eapply Hdis5 ]; [| now sets ].
+                   rewrite !Union_assoc. rewrite Union_commut. rewrite <- Union_Included_Union_Setminus.
+                   now sets. now tci.  eapply Included_trans. eapply name_in_fundefs_bound_var_fundefs. now sets.
+            + eassumption. }
         
         simpl. intros u w1 [Hyp Hyp']. split. eapply Hyp'. eassumption. }
 
@@ -1921,11 +2010,9 @@ Section Inline_correct.
            rewrite apply_r_list_eq; eauto. eapply Union_Included. now sets. 
            eapply Included_Union_preserv_l. rewrite <- Same_set_all_fun_name.
            rewrite Setminus_Union_distr. rewrite !image_Union. eapply Union_Included. now sets.
-
            eapply Included_trans. eapply image_monotonic. eapply Included_Setminus_compat.
-           eapply occurs_free_fun_map_add_fundefs. reflexivity.
-           rewrite !Setminus_Union_distr. rewrite Setminus_Same_set_Empty_set. normalize_sets. rewrite image_Union.
-           xsets. 
+           eapply occurs_free_fun_map_add_fundefs. reflexivity. rewrite !Setminus_Union_distr, Setminus_Same_set_Empty_set.
+           normalize_sets. rewrite !image_Union. xsets. 
         -- eapply Included_trans. eapply Included_Setminus_compat. eassumption. reflexivity.
            eapply Setminus_Included_Included_Union. 
            eapply Included_trans. eapply image_apply_r_set_list. now eauto.
@@ -1974,7 +2061,7 @@ Section Inline_correct.
                 -- eapply Disjoint_Included_r. eassumption.
                    eapply Disjoint_Included_l. eapply image_apply_r_set_list. now eauto.
                    eapply Union_Disjoint_l. now sets. rewrite <- Same_set_all_fun_name.
-                   eapply Disjoint_sym. eapply Disjoint_Included; [| | eapply Hdis2 ].
+                   eapply Disjoint_sym. eapply Disjoint_Included; [| | eapply Hdis3 ].
                    normalize_occurs_free. now xsets. now sets.
               * assert (Hdisys : Disjoint positive (FromList ys1)
                                           (occurs_free_fundefs f2 :|: name_in_fundefs f2
@@ -1987,45 +2074,40 @@ Section Inline_correct.
                 eapply fun_map_inv_antimon. eapply fun_map_inv_set_lists; [ | | | now eauto ].
                 eapply fun_map_inv_set_lists_r; [| | now eauto ]. 
                 -- rewrite <- Hseq. rewrite <- H14. eapply fun_map_inv_sig_extend_Disjoint.
-
                    eapply fun_map_inv_def_funs_add_fundefs. eapply fun_map_inv_i_mon. eassumption. omega.
-                   ++ rewrite H14, Hseq. eapply preord_env_P_inj_antimon. eapply IHi. eassumption. omega.
-                      normalize_occurs_free. sets.
+                   ++ eapply preord_env_P_inj_antimon. rewrite apply_r_list_eq in H14.
+                      rewrite H14. eapply IHi. omega. omega. eassumption. now eauto. normalize_occurs_free. sets.
                    ++ eassumption.
                    ++ normalize_occurs_free. sets.
                    ++ eapply Disjoint_Included; [| | eapply Hdis1 ]. now sets. normalize_bound_var.
                       eapply Included_trans. eapply name_in_fundefs_bound_var_fundefs. now sets.
-                   ++ rewrite Same_set_all_fun_name, H14, Hseq. eapply Disjoint_Included ; [| | eapply Hdis2 ]. now sets. eassumption.
-                   ++ eapply Disjoint_Included_r. eapply occurs_free_fun_map_add_fundefs.
-                      rewrite Union_commut. rewrite Union_assoc. eapply Union_Disjoint_r.
-                      ** sets.
-                      ** sets.
+                   ++ rewrite Same_set_all_fun_name, H14, Hseq. eapply Disjoint_Included ; [| | eapply Hdis3 ]. now sets. eassumption.
+                   ++ eapply Disjoint_Included_r. eapply occurs_free_fun_map_add_fundefs. sets.
                 -- rewrite image_f_eq_subdomain.
                    2:{ rewrite apply_r_set_list_f_eq. eapply f_eq_subdomain_extend_lst_Disjoint.
-                       eapply Disjoint_Included_r. eapply occurs_free_fun_map_add_fundefs.
-                      rewrite Union_commut. rewrite Union_assoc. eapply Union_Disjoint_r.
-                      sets. sets. }
-                   
-                   eapply Disjoint_Included_r.  
+                       eapply Disjoint_Included_r. eapply occurs_free_fun_map_add_fundefs. sets. }                   
+                   eapply Disjoint_Included_r. 
                    eapply image_apply_r_set_list. now eauto. eapply Union_Disjoint_r. 
                    eapply Disjoint_Included_l. eassumption. now sets.
                    rewrite <- Same_set_all_fun_name. 
                    eapply Disjoint_Included_l. eassumption.
-                   eapply Disjoint_Included; [| | eapply Hdis2 ]. normalize_occurs_free.
-                   ++ eapply Included_Union_preserv_r. eapply image_monotonic. eapply Setminus_Included_Included_Union.
-                      eapply Included_trans. eapply occurs_free_fun_map_add_fundefs. sets.
-                   ++ sets.
+                   eapply Disjoint_Included; [| | eapply Hdis3 ]. normalize_occurs_free.
+                   eapply Included_trans. eapply image_monotonic. eapply Included_Setminus_compat. eapply occurs_free_fun_map_add_fundefs. reflexivity.
+                   rewrite !Setminus_Union_distr. rewrite Setminus_Same_set_Empty_set. normalize_sets.
+                   now sets. now sets.
                 -- eapply unique_bindings_fun_in_fundefs. eapply find_def_correct. eassumption. eassumption.
                 -- eapply Union_Disjoint_r.
                    ++ eapply Disjoint_Included_r. eapply occurs_free_fun_map_add_fundefs. now sets.
-                   ++ rewrite Dom_map_add_fundefs. eapply Union_Disjoint_r. sets.
-                      admit. (* lemmas about fun_map_names *)
+                   ++ rewrite Dom_map_add_fundefs. eapply Union_Disjoint_r. now sets.
+                      eapply Disjoint_Included; [| | eapply Hdis4 ]. now sets. repeat normalize_bound_var.
+                      eapply Included_Union_preserv_l.  
+                      eapply Included_trans; [| eapply fun_in_fundefs_bound_var_fundefs; eapply find_def_correct; eauto ]. now sets.
                 -- normalize_occurs_free. sets.
           - inv HIn. contradiction. rewrite def_funs_neq in Hgetx; [| eassumption ]. eapply Henv in Hgetx; [| eassumption ]. destructAll. 
             eexists. rewrite apply_r_set_list_f_eq. rewrite extend_lst_gso. rewrite def_funs_neq. 
             split; eauto. eapply preord_val_monotonic. eassumption. omega. 
             + intros Hc. eapply Same_set_all_fun_name in Hc. rewrite H14 in Hc. 
-              rewrite apply_r_list_eq in Hc; [| | now eauto ]. eapply Hdis2. constructor. 
+              rewrite apply_r_list_eq in Hc; [| | now eauto ]. eapply Hdis3. constructor. 
               2:{ right. eapply In_image. eauto. } 
               eapply fresh_Range. 2:{ eapply Hsub. eassumption. } eassumption. eassumption.
             + rewrite <- Same_set_all_fun_name. intros Hc. eapply Hdis1. constructor. normalize_bound_var. left.
@@ -2039,7 +2121,7 @@ Section Inline_correct.
            eapply Disjoint_Included_l. eapply name_in_fundefs_bound_var_fundefs.
            eapply Disjoint_Included; [| | eapply Hdis1 ]. now sets. normalize_bound_var. now sets.
 
-           rewrite Same_set_all_fun_name, H14, Hseq. eapply Disjoint_Included; [| | eapply Hdis2 ]. now sets. eassumption.
+           rewrite Same_set_all_fun_name, H14, Hseq. eapply Disjoint_Included; [| | eapply Hdis3 ]. now sets. eassumption.
            normalize_occurs_free. rewrite !Union_assoc. rewrite Union_Setminus_Included. now sets. tci. now sets.
     - (* Eapp *)
       simpl. destruct (update_App St IH v t (apply_r_list sig l) st) as [s b] eqn:Hup. 
@@ -2064,9 +2146,11 @@ Section Inline_correct.
                        (negb str_flag || straight_code e)) eqn:Hbeq.
              { eapply andb_true_iff in Hbeq. inv Hbeq. symmetry in H. eapply beq_nat_eq in H.
                eapply orb_true_iff in H0.
-               eapply bind_triple. 
-               eapply click_spec2 with (P := fun s => fresh S (next_var s)). 
-               intros _x w.               
+               edestruct Hfm. eassumption. destructAll.
+
+               eapply bind_triple. eapply click_spec2 with (P := fun s => fresh S (next_var s)). 
+               intros _u w.
+
                edestruct Hfm. eassumption. destructAll.
 
                eapply pre_strenghtening with
@@ -2074,9 +2158,9 @@ Section Inline_correct.
                now clear; firstorder. 
                
                eapply post_weakening; [|  eapply frame_rule; eapply IHd; try omega ].
+
                ++ simpl. intros. destructAll.  
                   split; [| split; [| split; [| split; [| split; [| split; [| split ]]]]]]; try eassumption.
-
                   ** congruence.
                   ** eapply Included_trans. eassumption. 
                      eapply Included_trans. eapply image_apply_r_set_list.
@@ -2088,16 +2172,16 @@ Section Inline_correct.
                      eapply image_monotonic. eapply occurs_free_fun_map_get. eassumption.
                      eapply image_monotonic. eapply Included_trans. eapply Setminus_Included.
                      eapply occurs_free_fun_map_remove. 
-                  ** rewrite H8. eassumption.
-                  ** eauto.
-                  ** intros Heq _. inv H0. simpl in *. congruence. eauto. eapply H16; eauto.
+                  ** rewrite H18. eauto.
+                  ** exact I.
+                  ** intros Heq _. inv H0. simpl in *. congruence. eapply H25; eauto.
                   ** intros. eapply preord_exp_app_l.
                      --- eauto.
                      --- eauto.
-                     --- intros. assert (Hf' := H20). assert (Heqf' := Heqf).
-                         edestruct H20; eauto. destructAll.
-                         do 2 subst_exp. eapply H17.
-                         +++ edestruct preord_env_P_inj_get_list_l. now eapply H19. normalize_occurs_free. now sets.
+                     --- intros. assert (Hf' := H29). assert (Heqf' := Heqf).
+                         edestruct H29; eauto. destructAll.
+                         do 2 subst_exp. eapply H26.
+                         +++ edestruct preord_env_P_inj_get_list_l. now eapply H28. normalize_occurs_free. now sets.
                              eassumption. destructAll.                           
                              eapply preord_env_P_inj_set_lists_l'; try eassumption.
                          +++ eapply fun_map_inv_antimon. eapply fun_map_inv_set_lists; [ | | | eassumption ].
@@ -2114,28 +2198,28 @@ Section Inline_correct.
                ++ eapply Disjoint_Included_r. eapply image_apply_r_set_list.
                   unfold apply_r_list. rewrite list_length_map. eassumption.
                   eapply Union_Disjoint_r.
-                  eapply Disjoint_Included; [ | | eapply Hdis1' ]. normalize_occurs_free.
+                  eapply Disjoint_Included; [ | | eapply Hdis2 ]. normalize_occurs_free.
                   rewrite !image_Union. rewrite FromList_apply_list. now sets.
                   eapply Included_Union_preserv_r. 
                   eapply Union_Included; [| now eapply bound_var_fun_map_remove ]. 
                   eapply Included_trans; [| eapply bound_var_fun_map_get; eauto ]. now sets.
                   rewrite Setminus_Union_distr. rewrite !image_Union. eapply Union_Disjoint_r.
-                  eapply Disjoint_Included; [| | eapply Hdis1' ].
+                  eapply Disjoint_Included; [| | eapply Hdis2 ].
                   eapply image_monotonic. eapply Included_Union_preserv_r.
                   eapply occurs_free_fun_map_get. eassumption.
                   eapply Included_Union_preserv_r.
                   eapply Union_Included; [| now eapply bound_var_fun_map_remove ].
                   eapply Included_trans; [| eapply bound_var_fun_map_get; eauto ]. now sets.
-                  eapply Disjoint_Included; [| | eapply Hdis1' ]. eapply image_monotonic. eapply Included_Union_preserv_r.
+                  eapply Disjoint_Included; [| | eapply Hdis2 ]. eapply image_monotonic. eapply Included_Union_preserv_r.
                   eapply Included_trans. eapply Setminus_Included. now eapply occurs_free_fun_map_remove.
                   eapply Included_Union_preserv_r. eapply Union_Included; [| now eapply bound_var_fun_map_remove ].
                   eapply Included_trans; [| eapply bound_var_fun_map_get; eauto ]. now sets.
                ++ eapply Union_Disjoint_r.
                   eapply Union_Disjoint_r. now sets.
-                  clear H7. eapply Disjoint_Included_r. eapply bound_var_fun_map_remove. now sets.
+                  clear H8. eapply Disjoint_Included_r. eapply bound_var_fun_map_remove. clear H16. now sets.
                   eapply Disjoint_Included_r. eapply image_apply_r_set_list.
                   unfold apply_r_list. rewrite list_length_map. eassumption.
-                  eapply Disjoint_Included_r; [ | eapply Hdis2 ]. normalize_occurs_free.
+                  eapply Disjoint_Included_r; [ | eapply Hdis3 ]. normalize_occurs_free.
                   rewrite FromList_apply_list.
                   eapply Union_Included; [ now sets  | ].
                   rewrite Setminus_Union_distr. eapply Included_Union_preserv_r. eapply image_monotonic.
@@ -2144,6 +2228,7 @@ Section Inline_correct.
                   eapply occurs_free_fun_map_get. eassumption.
                   eapply Included_trans. eapply Setminus_Included. eapply occurs_free_fun_map_remove. 
                ++ rewrite Dom_map_remove. sets.
+               ++ sets.
                ++ eapply fun_map_vars_inv_remove. 
                  (* Make lemma if needed about fun_map_vars fm S (set_list (combine xs (apply_r_list sig l)) sig) *)
                   intros ? ? ? ? ?. edestruct Hfm; eauto. destructAll.
@@ -2151,7 +2236,7 @@ Section Inline_correct.
                   eapply Disjoint_Included_r. eapply image_apply_r_set_list.
                   unfold apply_r_list. rewrite list_length_map. eassumption.
                   eapply Union_Disjoint_r.
-                  eapply Disjoint_Included_r; [| eapply Hdis2 ]. normalize_occurs_free.
+                  eapply Disjoint_Included_r; [| eapply Hdis3 ]. normalize_occurs_free.
                   rewrite image_Union. rewrite FromList_apply_list. now sets. now sets. }
              { eapply return_triple. 
                intros. split; [| split; [| split; [| split; [| split; [| split; [| split ]]]]]]; try eassumption.
@@ -2206,17 +2291,18 @@ Section Inline_correct.
         eapply Disjoint_Singleton_r. eassumption.
       + repeat normalize_bound_var_in_ctx. repeat normalize_occurs_free_in_ctx.
         eapply Disjoint_Included_r. eapply image_apply_r_set. eapply Union_Disjoint_r.
-        eapply Disjoint_sym. eapply Disjoint_Included; [| | eapply Hdis2 ]. now sets. now sets.
-        rewrite Setminus_Union_distr. eapply Disjoint_Included; [| | eapply Hdis1' ]. now sets. now sets.
+        eapply Disjoint_sym. eapply Disjoint_Included; [| | eapply Hdis3 ]. now sets. now sets.
+        rewrite Setminus_Union_distr. eapply Disjoint_Included; [| | eapply Hdis2 ]. now sets. now sets.
       + eapply Disjoint_Included_r.
         eapply Included_Union_compat. reflexivity.
         eapply image_apply_r_set. 
         repeat normalize_bound_var_in_ctx. repeat normalize_occurs_free_in_ctx.
         eapply Union_Disjoint_r. now sets.
         eapply Union_Disjoint_r. now sets.
-        eapply Disjoint_Included; [| | eapply Hdis2 ].
+        eapply Disjoint_Included; [| | eapply Hdis3 ].
         rewrite Setminus_Union_distr. rewrite !image_Union. now xsets. now sets.
       + eapply Disjoint_Included_l; [| eassumption ]. normalize_bound_var. sets.
+      + eapply Disjoint_Included_r. eapply bound_var_occurs_free_Eprim_Included. eassumption.
       + eapply fun_map_vars_set. eassumption.
       + intros e' w2. eapply return_triple.
         intros _ st'. intros [Hf1 [Hf2 [Hf3 [Hf4 [Hun [Hsub [Hsub' [Hsh [Hstr Hsem]]]]]]]]].
@@ -2254,9 +2340,8 @@ Section Inline_correct.
         eapply H0. now constructor.
     - (* Fcons *)
       simpl. 
-      eapply bind_triple. eapply pre_transfer_r.
-      now eapply get_fresh_names_spec. intros xs w. simpl.
-      eapply pre_curry_l. intros HSin. eapply pre_curry_l. intros Hf'. eapply pre_curry_l. intros Hnd.  eapply pre_curry_l. intros Hlen.
+      eapply bind_triple. eapply pre_transfer_r. now eapply get_fresh_names_spec. intros xs w. simpl.
+      eapply pre_curry_l. intros HSin. eapply pre_curry_l. intros Hf'. eapply pre_curry_l. intros Hnd. eapply pre_curry_l. intros Hlen.
       eapply bind_triple. 
       { do 2 eapply frame_rule. eapply IHe with (S := S \\ FromList xs).
         - eassumption.
@@ -2265,31 +2350,48 @@ Section Inline_correct.
             now left. constructor; eauto. eapply Disjoint_Included; [| | eapply Hdis1 ]. now sets. now sets.
           + eapply Disjoint_Included_r. eapply Included_Union_Setminus with (s2 := name_in_fundefs (Fcons v t l e f5)). now tci.
             eapply Union_Disjoint_r.
-            eapply Disjoint_Included; [| | eapply Hdis1 ]. now sets. normalize_bound_var. now sets.
+            eapply Disjoint_Included; [| | eapply Hdis1 ]. eapply Included_Union_preserv_r. eapply Included_Setminus_compat.
+            eapply occurs_free_fun_map_remove. reflexivity. normalize_bound_var. now sets.
             eapply unique_bindings_fun_in_fundefs. now left. constructor; eauto.
         - repeat normalize_bound_var_in_ctx.
-          (* eapply Disjoint_Included; [| | eapply Hdis2 ]; now sets. *)
+          (* eapply Disjoint_Included; [| | eapply Hdis3 ]; now sets. *)
           eapply Disjoint_Included_r. eapply image_apply_r_set_list. now eauto.
           eapply Union_Disjoint_r.
-          eapply Disjoint_sym. eapply Disjoint_Included; [| | eapply Hdis2 ]; now sets.
-          rewrite FromList_apply_list in Hnames2. rewrite <- Same_set_all_fun_name in Hnames2.
-          eapply Disjoint_Included_r. eapply Included_Union_Setminus with (s2 := image (apply_r sig) (name_in_fundefs (Fcons v t l e f5))).
-          now tci. eapply Union_Disjoint_r. eapply Disjoint_Included_r. eapply image_Setminus. now tci. rewrite Setminus_Union_distr. 
-          eapply Disjoint_Included; [| | eapply Hdis1' ]. rewrite !Setminus_Union_distr. normalize_occurs_free.
-          rewrite !Setminus_Union. eapply image_monotonic. eapply Union_Included. simpl. now sets. now sets. now sets. 
-          now xsets.
-        - eapply Union_Disjoint_r. repeat normalize_bound_var_in_ctx. now xsets.
+          + eapply Union_Disjoint_l.
+            * eapply Disjoint_sym. eapply Disjoint_Included; [| | eapply Hdis3 ]; now sets.
+            * eapply Disjoint_Included_l. eapply bound_var_fun_map_remove.
+              eapply Disjoint_sym. eapply Disjoint_Included; [| | eapply Hdis3 ]; now sets.
+          + rewrite FromList_apply_list in Hnames2. rewrite <- Same_set_all_fun_name in Hnames2.
+            eapply Disjoint_Included_r. eapply Included_Union_Setminus with (s2 := image (apply_r sig) (name_in_fundefs (Fcons v t l e f5))).
+            now tci. eapply Union_Disjoint_r. eapply Disjoint_Included_r. eapply image_Setminus. now tci. rewrite Setminus_Union_distr. 
+            eapply Disjoint_Included; [| | eapply Hdis2 ]. rewrite !Setminus_Union_distr. normalize_occurs_free.
+            rewrite !Setminus_Union. eapply image_monotonic. eapply Union_Included. simpl. now sets.
+            eapply Included_trans. eapply Setminus_Included. eapply Included_trans. eapply occurs_free_fun_map_remove. now sets.
+            eapply Union_Included. now sets. eapply Included_trans. eapply bound_var_fun_map_remove. now sets.
+            eapply Union_Disjoint_l. now xsets.
+            eapply Disjoint_Included_l. eapply bound_var_fun_map_remove. now sets. 
+        - eapply Union_Disjoint_r. repeat normalize_bound_var_in_ctx.
+          eapply Union_Disjoint_r. now xsets. eapply Disjoint_Included_r. eapply bound_var_fun_map_remove. now sets. 
+
           eapply Disjoint_Included_r. eapply image_apply_r_set_list. now eauto.
           eapply Union_Disjoint_r. now sets.
           eapply Disjoint_Included_r. eapply Included_Union_Setminus with (s2 := image (apply_r sig) (name_in_fundefs (Fcons v t l e f5))).
           now tci. eapply Union_Disjoint_r. eapply Disjoint_Included_r. eapply image_Setminus. now tci. rewrite Setminus_Union_distr. 
-          eapply Disjoint_Included; [| | eapply Hdis2 ]. rewrite !Setminus_Union_distr. normalize_occurs_free.
+          eapply Disjoint_Included; [| | eapply Hdis3 ]. rewrite !Setminus_Union_distr. normalize_occurs_free.
           rewrite !Setminus_Union. eapply Included_Union_preserv_r. eapply image_monotonic. eapply Union_Included. simpl.
-          now sets. now sets. now sets. eapply Disjoint_Included; [| | eapply Hnames2 ]. rewrite FromList_apply_list. rewrite Same_set_all_fun_name.
+          now sets.
+          eapply Included_trans. eapply Setminus_Included. eapply Included_trans. eapply occurs_free_fun_map_remove. now sets. now sets.
+
+          eapply Disjoint_Included; [| | eapply Hnames2 ]. rewrite FromList_apply_list. rewrite Same_set_all_fun_name.
           reflexivity. now sets.
-        - admit. (* funnames_in_exp lemmas *)
+        - repeat normalize_bound_var_in_ctx. rewrite Dom_map_remove.
+          eapply Disjoint_Included; [| | eapply Hdis4 ]; sets.
+          rewrite !Setminus_Union_distr. do 2 eapply Included_Union_preserv_r. eapply Included_Union_preserv_l.
+          rewrite Setminus_Disjoint. reflexivity. simpl. eapply Union_Disjoint_r. now sets.
+          eapply Disjoint_Included_r; [| eapply H8 ]. eapply name_in_fundefs_bound_var_fundefs. 
+        - eapply Hdis5. now left.
         - repeat normalize_occurs_free_in_ctx. repeat normalize_bound_var_in_ctx.
-          eapply fun_map_vars_set_list. eassumption. }
+          eapply fun_map_vars_set_list. eapply fun_map_vars_inv_remove. eassumption. }
 
       intros e' w'. simpl. eapply pre_curry_l. intros Hxs. eapply pre_curry_l; intros Hleq1.     
       eapply bind_triple.
@@ -2303,20 +2405,20 @@ Section Inline_correct.
               simpl. rewrite Setminus_Union. now sets. now sets. now sets. 
             + eapply Disjoint_Included_r. eapply Included_Union_Setminus with (s2 := image (apply_r sig) [set v]). now tci.
               eapply Union_Disjoint_r. eapply Disjoint_Included_r. eapply image_Setminus. now tci. rewrite !Setminus_Union_distr.
-              eapply Disjoint_Included; [| | eapply Hdis1' ]. normalize_occurs_free. now sets. normalize_bound_var. now sets.
+              eapply Disjoint_Included; [| | eapply Hdis2 ]. normalize_occurs_free. now sets. normalize_bound_var. now sets.
               eapply Disjoint_Included; [| | eapply Hnames2 ]. rewrite FromList_apply_list, <- Same_set_all_fun_name. simpl. now sets.
               normalize_bound_var. now sets.
             + repeat normalize_bound_var_in_ctx. repeat normalize_occurs_free_in_ctx. 
               eapply Union_Disjoint_r. 
-              eapply Disjoint_Included; [| | eapply Hdis2 ]; now sets.
+              eapply Disjoint_Included; [| | eapply Hdis3 ]; now sets.
               eapply Disjoint_Included_r. eapply Included_Union_Setminus with (s2 := image (apply_r sig) [set v]). now tci.
               eapply Union_Disjoint_r. 
               eapply Disjoint_Included_r. eapply image_Setminus. now tci.
-              eapply Disjoint_Included; [| | eapply Hdis2 ]. eapply Included_Union_preserv_r.
+              eapply Disjoint_Included; [| | eapply Hdis3 ]. eapply Included_Union_preserv_r.
               eapply image_monotonic. rewrite !Setminus_Union_distr. now sets. now sets.
               eapply Disjoint_Included; [| | eapply Hnames2 ]. rewrite FromList_apply_list, <- Same_set_all_fun_name. simpl. now sets. now sets.
-            + repeat normalize_bound_var_in_ctx. repeat normalize_occurs_free_in_ctx. sets.
-              admit. (* funnames_in_exp lemmas *)
+            + repeat normalize_bound_var_in_ctx. repeat normalize_occurs_free_in_ctx. xsets.
+            + intro; intros. eapply Hdis5. right. eassumption.
             + eapply fun_map_vars_antimon; eauto. sets.
             + simpl in Hnames1. inv Hnames1. eassumption.
             + eapply Disjoint_Included; [ | | eapply Hnames2 ]; simpl; sets. normalize_sets. sets. normalize_bound_var. now sets. } 
@@ -2361,7 +2463,9 @@ Section Inline_correct.
              eapply Included_trans. eapply Setminus_Included. eapply Included_trans.
              rewrite <- image_Singleton, <- image_Union. eapply image_Setminus. now tci.
              rewrite !Setminus_Union_distr, !Setminus_Union. normalize_occurs_free.
-             rewrite !image_Union. eapply Union_Included; xsets.
+             rewrite !image_Union. eapply Union_Included; sets. now xsets.
+             eapply Included_trans. eapply image_monotonic. eapply Included_trans. eapply Setminus_Included.
+             eapply occurs_free_fun_map_remove. now sets.
           -- rewrite <- image_Singleton. eapply Included_trans. eapply image_Setminus. now tci.
              rewrite Setminus_Union_distr. normalize_occurs_free. sets.             
       + normalize_bound_var. simpl. rewrite Setminus_Union_distr. eapply Union_Included. now sets.
@@ -2385,7 +2489,7 @@ Section Inline_correct.
                 eapply preord_env_P_inj_antimon. eassumption. eapply Included_trans.
                 eapply occurs_free_in_fun with (B := (Fcons v ft xs0 e1 f5)). now left.
                 sets.
-             ++ eapply fun_map_inv_antimon. eassumption.
+             ++ eapply fun_map_inv_remove. eapply fun_map_inv_antimon. eassumption.
                 eapply Included_trans. eapply occurs_free_in_fun with (B := (Fcons v ft xs0 e1 f5)). now left.
                 sets.
         * edestruct H15. eassumption. destructAll.
@@ -2414,6 +2518,7 @@ Section Inline_correct.
       + intros. inv H0.
   Qed.
 
+   
   Lemma apply_r_empty_f_eq : 
     f_eq (apply_r (M.empty var)) id.
   Proof.
@@ -2435,12 +2540,13 @@ Section Inline_correct.
   Qed.
   
 
-  Lemma inline_correct_top d (Hleq : (d <= G)%nat) P (e : exp) (st : St) (c:comp_data) (Hi : inclusion (P1 d) P):
+  Lemma inline_correct_top d (Hleq : (d <= G)%nat) P (e : exp) (st : St) (c:comp_data) (Hi : inclusion (P1 d) P) z :
     unique_bindings e ->
     Disjoint _ (bound_var e) (occurs_free e) ->
-    (max_var e 1%positive) < (next_var c) ->
+    (* (* this assumption can probably be relaxed because inlining renames all binders, but I don't want to change the main proof *) *)
+    (* (max_var e 1%positive) < (next_var c) ->  *)
     exists e' c',
-      beta_contract_top St IH e d st c true  = (Ret e', c') /\
+      inline_top St IH z e d st c true  = (Ret e', c') /\
       unique_bindings e' /\
       occurs_free e' \subset occurs_free e /\
       Disjoint _ (bound_var e') (occurs_free e') /\
@@ -2450,8 +2556,8 @@ Section Inline_correct.
           preord_env_P cenv PG (occurs_free e) k rho1 rho2 ->
           preord_exp cenv P PG k (e, rho1) (e', rho2)).
   Proof.
-    intros. edestruct (inline_correct_mut d) as [He _].
-    unfold beta_contract_top, triple in *. eassumption.
+    intros. edestruct (inline_correct_mut d) as [He _]. eassumption.
+    unfold inline_top, triple in *.
     
     specialize (He e (M.empty _) (M.empty _) st (fun x => max_var e 1%positive < x) true H).
 
@@ -2467,9 +2573,9 @@ Section Inline_correct.
     assert (Hdis1 : Disjoint var (fun x : var => max_var e 1 < x)
                              (bound_var e :|: image (apply_r (M.empty var)) (occurs_free e))).
     { rewrite apply_r_empty_f_eq. rewrite image_id.  
-      constructor. intros x Hnin. inv Hnin. inv H3.
-      eapply bound_var_leq_max_var with (y := 1%positive) in H4. unfold Ensembles.In in *. zify. omega.
-      eapply occurs_free_leq_max_var with (y := 1%positive) in H4. unfold Ensembles.In in *. zify. omega. }
+      constructor. intros x Hnin. inv Hnin. inv H2.
+      eapply bound_var_leq_max_var with (y := 1%positive) in H3. unfold Ensembles.In in *. zify. omega.
+      eapply occurs_free_leq_max_var with (y := 1%positive) in H3. unfold Ensembles.In in *. zify. omega. }
     
 
     
@@ -2482,12 +2588,21 @@ Section Inline_correct.
     assert (Hfinv : fun_map_vars (M.empty (fun_tag * list var * exp))
                                  (fun x : var => max_var e 1 < x)
                                  (M.empty var)).
-    { unfold fun_map_vars. intros. rewrite M.gempty in H2. inv H2. }
-    
-    assert (Hf' : fresh (fun x : var => max_var e 1 < x) (next_var (fst (c, tt)))).
-    { unfold fresh. intros. unfold Ensembles.In in *. simpl in *. zify; omega. }
+    { unfold fun_map_vars. intros. rewrite M.gempty in H1. inv H1. }
 
-    specialize (He Hdis Hdis1 Hdis2 Hdis3 Hfinv tt (c, tt) Hf').
+    destruct (restart_names z e c) as [c_data nenv] eqn:Hnames.
+
+    assert (Hf' : fresh (fun x : var => max_var e 1 < x) (next_var (fst (c_data, (nenv, false))))).
+    { unfold fresh. intros. unfold Ensembles.In in *. simpl in *.
+      unfold restart_names in Hnames. destruct c. inv Hnames. simpl in H1.  reflexivity. simpl in Hnames.
+
+      zify; omega. }
+
+
+    assert (Heq : c_data = c).
+    { unfold restart_names in Hnames. destruct c. inv Hnames. reflexivity. simpl in Hnames. 
+    
+    specialize (He Hdis Hdis1 Hdis2 Hdis3 Hfinv tt (c_data, (false, nenv))).  Hf').
     
     unfold runState, run_compM. simpl in *. 
     
